Filling in holes. Minor change to recoding structure.

SAW/spec/EC/Coq/CryptoToCoq_equiv.v
@@ -21,6 +21,9 @@ Import SAWCorePrelude.
 From CryptolToCoq Require Import SAWCoreBitvectors.
 From CryptolToCoq Require Import Everything.
 
+From Bits Require Import operations.
+From Bits Require Import operations.properties.
+
 Ltac ecSimpl_one :=
   match goal with
     | [ |- context[ecNumber (TCNum ?a) ?t (PLiteralSeqBool (TCNum ?s))]] =>
@@ -403,7 +406,7 @@ Theorem toList_drop_equiv : forall A (inh : Inhabited A) n1 n2 ls,
 
 Admitted.
 
-Theorem nth_order_S_cons : forall (A : Type) a n (v : Vec (S n) A) (pf : (S n < S (S n))%nat)(pf' : (n < S n)%nat),
+Theorem nth_order_S_cons : forall (A : Type) a n (v : Vec n A) n' (pf : (S n' < S n)%nat)(pf' : (n' < n)%nat),
   nth_order (Vector.cons _ a _ v) pf = nth_order v pf'.
 
   intros.
@@ -455,7 +458,7 @@ Theorem lsb_0_even_h : forall n (v : Vec n _) acc (pf : (pred n < n)%nat),
   apply ssr_double_even.
 
   assert (n < S n)%nat by lia.
-  rewrite (@nth_order_S_cons _ _ _ _ _ H0) in H.
+  rewrite (@nth_order_S_cons _ _ _ _ _ _ H0) in H.
   eapply IHn.
   eauto.
 
@@ -495,7 +498,7 @@ Theorem lsb_1_not_even_h : forall n (v : Vec n _) acc (pf : (pred n < n)%nat),
   reflexivity.
 
   assert (n < S n)%nat by lia.
-  rewrite (@nth_order_S_cons _ _ _ _ _ H0) in H.
+  rewrite (@nth_order_S_cons _ _ _ _ _ _ H0) in H.
   eapply IHn.
   eauto.
 
@@ -772,5 +775,645 @@ Theorem ne_false_impl_true : forall a,
   intuition idtac.
 
 Qed.
+
+Theorem bvToNat_toZ_equiv : forall n x,
+  (BinInt.Z.of_nat (bvToNat n x)) = bvToInt n x.
+Admitted.
+
+Theorem sbvToInt_bvToInt_id : forall n x,
+  intToBv n (sbvToInt n x) = x.
+Admitted.
+
+Theorem ecEq_bv_true : forall n v,  
+  ecEq (bitvector n) (PEqWord n) v v = true.
+
+  intros.
+  apply bvEq_refl.
+
+Qed.
+
+Theorem ecEq_bv_false : forall n v1 v2,
+  v1 <> v2 ->
+  ecEq (bitvector n) (PEqWord n) v1 v2 = false.
+
+  intros.
+  unfold ecEq.
+  simpl.
+  case_eq (bvEq n v1 v2); intros; trivial.
+  apply bvEq_eq in H0.
+  intuition.
+Qed.
+
+Theorem ecEq_vec_bv_true : forall n1 n2 v,
+  (ecEq (Vec n1 (bitvector n2)) (PEqVec n1 (bitvector n2) (PEqWord n2)) v v) = true.
+
+  intros.
+  unfold ecEq.
+  simpl.
+  unfold vecEq.
+
+Admitted.
+
+Theorem ecEq_vec_bv_false : forall n1 n2 v1 v2,
+  v1 <> v2 ->
+  (ecEq (Vec n1 (bitvector n2)) (PEqVec n1 (bitvector n2) (PEqWord n2)) v1 v2) = false.
+
+Admitted.
+
+Theorem ecNotEq_vec_bv_false : forall n1 n2 v,
+  (ecNotEq (Vec n1 (bitvector n2)) (PEqVec n1 (bitvector n2) (PEqWord n2)) v v) = false.
+
+    intros.
+  unfold ecNotEq.
+  
+
+Admitted.
+
+Theorem ecNotEq_vec_bv_true : forall n1 n2 v1 v2,
+  v1 <> v2 ->
+  (ecNotEq (Vec n1 (bitvector n2)) (PEqVec n1 (bitvector n2) (PEqWord n2)) v1 v2) = true.
+Admitted.
+
+Theorem rep_false_eq_int_bv : forall n, (replicate n _ false) = (intToBv n 0).
+
+Admitted.
+
+Theorem ecOr_0_if : forall n x y, 
+    ecOr (bitvector n) (PLogicWord n) x y = (replicate n _ false) ->
+    (x = (replicate n _ false) /\ y = (replicate n _ false)).
+Admitted.
+
+Theorem fold_or_impl_0 : forall (n1 n2 : nat) x y,
+  ecFoldl n1 (CryptolPrimitivesForSAWCore.seq n2 Bool) (CryptolPrimitivesForSAWCore.seq n2 Bool) (ecOr (CryptolPrimitivesForSAWCore.seq n2 Bool) (PLogicSeqBool n2))
+     y x = intToBv n2 0 ->
+  (x = (replicate n1 _ (replicate n2 _ false)) /\ y = (replicate n2 _ false)).
+
+  induction n1; intros; simpl in *.
+  unfold replicate. simpl in *.
+  generalize H.
+  eapply (case0 (fun x => foldl (bitvector n2) (bitvector n2) 0%nat (ecOr (bitvector n2) (PLogicWord n2)) y x = intToBv n2 0 ->
+x = @Vector.nil (Vec n2 bool) /\ y = gen n2 bool (fun _ : Nat => false))); eauto; intuition.
+  simpl in *; subst.
+  rewrite <- rep_false_eq_int_bv.
+  trivial.
+
+  unfold replicate in *. simpl.
+  generalize H.
+  eapply (caseS' x); intuition;
+  simpl in *;
+  edestruct IHn1; eauto;
+  subst.
+  f_equal.
+  edestruct ecOr_0_if; eauto.
+  edestruct ecOr_0_if; eauto.
+
+Qed.
+
+Theorem scanl_gen_equiv : forall A n f1 f2 z1 x,
+  (SAWCoreVectorsAsCoqVectors.scanl Integer A n
+         (fun (z : A) (_ : Integer) =>
+          z1 z) x
+         (gen n Integer f1))
+  = 
+  (SAWCoreVectorsAsCoqVectors.scanl Integer A n
+         (fun (z : A) (_ : Integer) =>
+          z1 z) x
+         (gen n Integer f2)).
+
+  induction n; intuition; simpl in *.
+  f_equal.
+  apply IHn.
+Qed.
+
+Fixpoint bv64Nats_h (n : nat) v :=
+  match n with
+  | 0%nat => List.nil
+  | S n' => (intToBv 64%nat (Z.of_nat v)) :: (bv64Nats_h n' (S v))
+  end.
+
+Definition bv64Nats n := bv64Nats_h n 0.
+
+Theorem gen_nat_seq_eq_h : forall n v,
+  (to_list
+      (gen n (bitvector 64)
+         (fun i : nat => intToBv 64%nat (Z.of_nat (addNat i v%nat)))))
+  = bv64Nats_h n v.
+
+  induction n; intuition; simpl in *.
+  rewrite to_list_cons.
+  f_equal.
+  rewrite <- IHn.
+  f_equal.  
+  eapply gen_domain_eq.
+  intros.
+  rewrite (eqNatAddComm _ (S v)).
+  simpl.
+  rewrite eqNatAddComm.
+  trivial.
+Qed.
+
+Theorem gen_nat_seq_eq : forall n,
+  (to_list
+      (gen n (bitvector 64)
+         (fun i : nat => intToBv 64%nat (Z.of_nat (addNat i 0%nat)))))
+  = bv64Nats n.
+
+  intros.
+  apply gen_nat_seq_eq_h.    
+Qed.
+
+Fixpoint nats_h n v :=
+  match n with
+  | 0%nat => List.nil
+  | S n' => v :: (nats_h n' (S v))
+  end.
+
+Definition nats n := nats_h n 0.
+
+Theorem toN_int_excl_length : forall n, 
+  List.length (toN_excl_int n) = n.
+
+  induction n; intuition idtac; simpl in *.
+
+  rewrite app_length.
+  rewrite IHn.
+  simpl.
+  lia.
+
+Qed.
+
+Theorem toN_int_length : forall n, 
+  List.length (toN_int n) = (S n).
+
+  intros.
+  unfold toN_int.
+  rewrite app_length.
+  rewrite toN_int_excl_length.
+  simpl.
+  lia.
+
+Qed.
+
+Theorem scanl_fix_convert : forall (A1 A2 B1 B2: Type)
+  (conva : A2 -> A1)(convb : B2 -> B1)
+  (f1 : A1 -> A1)(f2 : A2 -> A2)
+  (fb1 : A1 -> B1)(fb2 : A2 -> B2)
+  (fc1 : A1 -> B1)(fc2 : A2 -> B2),
+  (forall a, fb1 (conva a) = convb (fb2 a)) ->
+  (forall a, (exists b, a = (f2 b)) -> fc1 (conva a) = convb (fc2 a)) ->
+  (forall a, (exists b, a = (f2 b)) -> f1 (conva a) = conva (f2 a)) ->
+  forall n a1 a2,
+  (exists b, a2 = (f2 b)) ->
+  a1 = (conva a2) ->
+  List.Forall2 (fun b1 b2 => b1 = convb b2)
+  (scanl_fix f1 fb1 fc1 n a1)
+  (scanl_fix f2 fb2 fc2 n a2).
+
+  induction n; intros; simpl in *; subst.
+  econstructor.
+
+  destruct n.
+  econstructor.
+  eauto.
+  econstructor.
+  eauto.
+  econstructor.
+
+  econstructor.
+  eauto.
+  eapply IHn.
+  eauto.
+  eauto.
+
+Qed.
+
+
+Theorem mod_drop_equiv : forall s1 m a,
+  (Z.modulo (bvToInt _ a) (Z.shiftl 1 (Z.of_nat m))) =
+  (bvToInt _ (drop Bool s1 m a)).
+
+  intros.
+  
+
+Admitted.
+
+
+Theorem bvToInt_sbvToInt_equiv : forall n v,
+  (n > 0)%nat ->
+  (bvToInt n v < Z.pow 2 (Z.of_nat (pred n)))%Z ->
+  (sbvToInt n v = bvToInt n v).
+
+  intros.
+  unfold sbvToInt, bvToInt, spec.toZ, spec.toPosZ.
+  destruct n. lia.
+  case_eq (spec.splitmsb (bvToBITS v)); intros.
+  destruct b0.
+
+Admitted.
+
+Theorem shiftR_bvToInt_nonneg : 
+  forall n s x,
+  (s > 0)%nat ->
+  (VectorDef.hd (shiftR (S n) bool false x s) = false).
+
+Admitted.
+
+
+
+Theorem bvToInt_drop_equiv : forall n1 n2 x,
+  ((bvToInt _ x) < Z.pow 2 (Z.of_nat n2))%Z ->
+  bvToInt _ (drop _ n1 n2 x) = bvToInt _ x.
+
+Admitted.
+
+
+Theorem sbvToInt_drop_equiv_h : forall n1 n2 x,
+  (-(Z.pow 2 (Z.of_nat (n2))) <= (sbvToInt _ x) < Z.pow 2 (Z.of_nat (n2)))%Z ->
+  spec.toZ (bvToBITS (drop _ n1 (S n2) x)) = sbvToInt _ x.
+
+Admitted.
+
+Theorem sbvToInt_drop_equiv : forall n1 n2 x,
+  (n2 > 0)%nat -> 
+  (-(Z.pow 2 (Z.of_nat (pred n2))) <= (sbvToInt _ x) < Z.pow 2 (Z.of_nat (pred n2)))%Z ->
+  sbvToInt _ (drop _ n1 n2 x) = sbvToInt _ x.
+
+  intros.
+  destruct n2.
+  lia.
+  unfold sbvToInt.
+  simpl in *.
+  rewrite sbvToInt_drop_equiv_h; trivial.
+
+Qed.
+
+Theorem sbvToInt_bvSub_equiv : forall n (v1 v2 : Vec n _),
+  (n > 1)%nat -> 
+    (-(Z.pow 2 (Z.of_nat (pred (pred n)))) <= (sbvToInt _ v1) < Z.pow 2 (Z.of_nat (pred (pred n))))%Z ->
+   (-(Z.pow 2 (Z.of_nat (pred (pred n)))) <= (sbvToInt _ v2) < Z.pow 2 (Z.of_nat (pred (pred n))))%Z ->
+  sbvToInt _ (bvSub v1 v2) = ((sbvToInt _ v1) - (sbvToInt _ v2))%Z.
+
+Admitted.
+
+Theorem bvToInt_intToBv_id : forall n v,
+  bvToInt n (intToBv n v) = v.
+
+Admitted.
+
+Theorem sbvToInt_intToBv_id : forall n v,
+  (-Z.pow 2 (Z.of_nat (pred n)) <= v < Z.pow 2 (Z.of_nat (pred n)))%Z ->
+  sbvToInt n (intToBv n v) = v.
+
+Admitted.
+
+Theorem sbvToInt_bvURem_equiv : forall n v1 v2,
+  (n > 0)%nat ->
+  (0 < bvToInt _ v2)%Z ->
+  (bvToInt _ v2 <= Z.pow 2 (Z.of_nat (pred n)))%Z ->
+  sbvToInt n (bvURem _ v1 v2) = Z.modulo (bvToInt _ v1) (bvToInt _ v2).
+
+  intros.
+  Local Transparent bvURem.
+  unfold bvURem.
+  destruct n. lia.
+  rewrite bvToInt_sbvToInt_equiv.
+  apply bvToInt_intToBv_id.
+  trivial.
+  rewrite bvToInt_intToBv_id.
+  eapply Z.lt_le_trans.
+  eapply Z.mod_pos_bound.
+  trivial.
+  trivial.
+Qed.
+
+Theorem bvToInt_drop_le : forall n1 n2 v,
+  (bvToInt _ (drop _ n1 n2 v) <= bvToInt _ v)%Z.
+
+Admitted.
+
+Theorem bvMul_2_shiftl_equiv : forall n v,
+  bvMul n (intToBv _ 2) v = shiftL _ _ false v 1.
+Admitted.
+
+Theorem shiftL_shiftL : forall (A : Type) n (b : A) v n1 n2,
+  (shiftL n _ b (shiftL n _ b v n1) n2) = shiftL n _ b v (n1 + n2).
+Admitted.
+
+Theorem bvToInt_shiftL_1_equiv : forall n s,
+  (s < n)%nat ->
+  bvToInt n (shiftL _ _ false (intToBv _ 1) s) = 
+  Z.shiftl 1 (Z.of_nat s).
+Admitted.
+
+Theorem sbvToInt_shiftL_1_equiv : forall n s,
+  (n > 0)%nat ->
+  (s < pred n)%nat ->
+  sbvToInt n (shiftL _ _ false (intToBv _ 1) s) = 
+  Z.shiftl 1 (Z.of_nat s).
+Admitted.
+
+Theorem bvToInt_bvSub_nonneg_equiv : forall n v1 v2,
+  (bvToInt _ v2 <= bvToInt _ v1)%Z ->
+  (bvToInt n (bvSub v1 v2)) =
+  ((bvToInt _ v1) - (bvToInt _ v2))%Z.
+Admitted.
+
+Theorem bvToBITS_bitsToBv_id : forall n v,
+  bvToBITS (@bitsToBv n v) = v.
+Admitted.
+
+Theorem toZ_toPosZ_equiv : forall n (v : spec.BITS (S n)),
+  (spec.toZ v mod 2 ^ Z.of_nat (S n) = spec.toPosZ v mod 2 ^ Z.of_nat (S n))%Z.
+Admitted.
+
+Theorem toPosZ_addB_equiv: forall n (v1 v2 : spec.BITS (S n)),
+  (0 <= spec.toPosZ v1 + spec.toZ v2 < Z.pow 2 (Z.of_nat (S n)))%Z ->
+  spec.toPosZ (addB v1 v2) =
+  (spec.toPosZ v1 + spec.toZ v2)%Z.
+
+  intros.
+  erewrite <- (@Zdiv.Zmod_small (spec.toPosZ v1 + spec.toZ v2)); eauto.
+  rewrite <- Zdiv.Zplus_mod_idemp_r.
+  rewrite toZ_toPosZ_equiv.
+  rewrite Zdiv.Zplus_mod_idemp_r.
+ 
+  rewrite addB_def.
+Admitted.
+
+
+Theorem sbvToInt_bvNeg_equiv : forall n v,
+  sbvToInt n (bvNeg _ v) = Z.opp (sbvToInt _ v).
+Admitted.
+
+Theorem bvToInt_bvAdd_small_equiv : forall n (v1 v2 : bitvector n),
+  (* (sbvToInt _ v2 <= bvToInt _ v1)%Z -> *)
+  (0 <= (bvToInt _ v1) + (sbvToInt _ v2) < Z.pow 2 (Z.of_nat n))%Z->
+  (bvToInt n (bvAdd _ v1 v2)) =
+  ((bvToInt _ v1) + (sbvToInt _ v2))%Z.
+
+  intros.
+  unfold bvToInt, sbvToInt in *.
+  destruct n.
+  (* empty bit vectors *)
+  admit.
+
+  Local Transparent bvAdd operations.adcB.
+  unfold bvAdd.
+  rewrite bvToBITS_bitsToBv_id.
+  apply toPosZ_addB_equiv.
+  apply H.
+
+Admitted.
+
+
+
+Theorem bvToInt_bvSub_small_equiv : forall n v1 v2,
+  (0 <= (bvToInt _ v1) - (sbvToInt _ v2) < Z.pow 2 (Z.of_nat n))%Z->
+  (bvToInt n (bvSub v1 v2)) =
+  ((bvToInt _ v1) - (sbvToInt _ v2))%Z.
+
+  intros.
+  rewrite bvSub_eq_bvAdd_neg.
+  rewrite <- Z.add_opp_r.
+  rewrite bvToInt_bvAdd_small_equiv.
+  rewrite sbvToInt_bvNeg_equiv.
+  reflexivity.
+  
+  rewrite sbvToInt_bvNeg_equiv.
+  rewrite Z.add_opp_r.
+  trivial.
+Qed.
+
+
+Theorem bvToInt_shiftR_lt : forall n v s b,
+  ((bvToInt n v) < (Z.pow 2 (Z.of_nat s + b)))%Z ->
+  ((bvToInt n (shiftR _ _ false v s)) < Z.pow 2 b)%Z.
+
+Admitted.
+
+Theorem bvToInt_nonneg : forall n v,
+  (0 <= bvToInt n v)%Z.
+Admitted.
+
+Theorem forall2_symm : forall (A B : Type)(P : B -> A -> Prop) lsa lsb,
+  List.Forall2 (fun a b => P b a) lsa lsb ->
+  List.Forall2 P lsb lsa.
+
+  induction 1; intros;
+  econstructor; eauto.
+
+Qed.
+
+Theorem forall2_trans : forall ( A B C : Type)(R1 : A -> B -> Prop)(R2 : B -> C -> Prop)(R3 : A -> C -> Prop)
+  lsa lsb lsc,
+  List.Forall2 R1 lsa lsb ->
+  (forall a b c, R1 a b -> R2 b c -> R3 a c) ->
+  List.Forall2 R2 lsb lsc ->
+  List.Forall2 R3 lsa lsc.
+
+  induction lsa; intuition; simpl in *.
+  inversion H; subst.
+  inversion H1; subst.
+  econstructor.
+
+  inversion H; subst.
+  inversion H1; subst.
+  econstructor.
+  eauto.
+  eapply IHlsa; eauto.
+
+Qed.
+
+Theorem forall2_eq : forall (A : Type)(ls1 ls2 : list A),
+  ls1 = ls2 ->
+  List.Forall2 eq ls1 ls2.
+
+  induction ls1; intros; simpl in *; subst.
+  econstructor.
+
+  econstructor; trivial.
+  eauto.
+
+Qed.
+
+Theorem forall2_map_eq : forall (A B : Type)(f : B -> A) lsa lsb,
+  List.Forall2 (fun a b => a = f b) lsa lsb ->
+  lsa = List.map f lsb.
+
+  induction 1; intros; simpl in *; trivial.
+  congruence.
+
+Qed.
+
+Theorem bvOr_bvToInt_equiv : forall n x y,
+  bvToInt n (bvOr x y) =
+  BinInt.Z.lor (bvToInt n x) (bvToInt n y).
+Admitted.
+
+Theorem bvSShr_intToBv_equiv : forall n z v,
+  bvSShr _ (intToBv (S n) z) v = intToBv (S n) (Z.shiftr z (Z.of_nat v)).
+Admitted.
+
+Theorem fold_left_unroll_one : forall (A B : Type) def (f : A -> B -> A) (ls : list B) a,
+  (List.length ls > 0)%nat ->
+  List.fold_left f ls a = List.fold_left f (List.tl ls) (f a (List.hd def ls)).
+
+  destruct ls; intros; simpl in *.
+  lia.
+  reflexivity.
+
+Qed.
+
+Theorem fold_left_R : forall (A1 A2 B1 B2 : Type)(RA : A1 -> A2 -> Prop)(RB : B1 -> B2 -> Prop)(f1 : A1 -> B1 -> A1)(f2: A2 -> B2 -> A2) ls1 ls2 a1 a2,
+  RA a1 a2 ->
+  List.Forall2 RB ls1 ls2 ->
+  (forall a1 a2 b1 b2, RA a1 a2 -> RB b1 b2 -> RA (f1 a1 b1) (f2 a2 b2)) ->
+  RA (List.fold_left f1 ls1 a1) (List.fold_left f2 ls2 a2).
+
+  induction ls1; destruct ls2; intros; simpl in *; trivial.
+  inversion H0.
+  inversion H0.
+  inversion H0; subst; clear H0.
+  eapply IHls1.
+  eapply H1; eauto.
+  trivial.
+  eauto.
+
+Qed.
+
+Theorem hd_rev_eq_last : forall (A : Type)(ls : list A)(def : A),
+  List.hd def (List.rev ls) = List.last ls def.
+
+  induction ls using rev_ind; intros; simpl in *; trivial.
+  rewrite rev_unit.
+  simpl.
+  rewrite last_last.
+  reflexivity.
+Qed.
+
+Theorem fold_left_scanl_app_equiv : forall (A B : Type) (f : A -> B -> A) ls def a1 a2,
+  a2 <> List.nil ->
+  List.fold_left
+(fun (x : list A) (y : B) =>
+ x ++ [f (List.last x def) y]) ls 
+(List.cons a1 a2) =
+  a1 :: (List.fold_left (fun (x : list A) (y : B) =>
+ x ++ [f (List.last x def) y]) ls 
+a2 ).
+
+  induction ls; intros; simpl in *; trivial.
+  rewrite (@IHls _ a1).
+  destruct a2.
+  intuition idtac.
+  reflexivity.
+  f_equal.
+  intuition idtac.
+  apply app_eq_nil in H0.
+  intuition idtac.
+
+Qed.
+
+Theorem fold_left_scanl_equiv : forall (A B : Type) def (f : A -> B -> A) ls a,
+  List.fold_left (fun x y => x ++ (f (List.last x def) y)::List.nil) ls [a] = 
+  CryptoToCoq_equiv.scanl f ls a.
+
+  induction ls; intros; simpl in *; trivial.
+  rewrite <- IHls.
+  rewrite fold_left_scanl_app_equiv.
+  reflexivity.
+  congruence.
+Qed.
+
+Theorem Forall2_scanl : forall (A1 A2 B1 B2 : Type)(PA : A1 -> A2 -> Prop)(PB : B1 -> B2 -> Prop)
+  (f1 : A1 -> B1 -> A1)(f2 : A2 -> B2 -> A2) ls1 ls2 a1 a2,
+  List.Forall2 PB ls1 ls2 ->
+  (forall a1 a2 b1 b2, PA a1 a2 -> PB b1 b2 -> PA (f1 a1 b1) (f2 a2 b2)) ->
+  PA a1 a2 ->
+  List.Forall2 PA (scanl f1 ls1 a1) (scanl f2 ls2 a2).
+
+  induction ls1; destruct ls2; simpl in *; intros.
+  econstructor; eauto.
+  inversion H.
+  inversion H.
+  inversion H; clear H; subst.
+  econstructor; eauto.
+
+Qed.
+
+Theorem Forall2_I : forall (A B : Type)(ls1 : list A)(ls2 : list B),
+  List.length ls1 = List.length ls2 ->
+  List.Forall2 (fun a b => True) ls1 ls2.
+
+  induction ls1; destruct ls2; intros; simpl in *; try lia.
+  econstructor.
+  econstructor; eauto; econstructor.
+
+Qed.
+
+Theorem Forall2_nth : forall (A B : Type)(P : A -> B -> Prop) lsa lsb,
+  List.Forall2 P lsa lsb ->
+  forall n defA defB,
+  P defA defB ->
+  P (List.nth n lsa defA) (List.nth n lsb defB).
+
+  induction 1; intros; simpl in *.
+  destruct n; trivial.
+  destruct n; trivial.
+  eapply IHForall2; trivial.
+
+Qed.
+
+Theorem bvNat_Z_to_nat_eq_intToBv : forall n (z : Z),
+  (0 <= z)%Z ->
+  bvNat n (Z.to_nat z) = intToBv n z.
+Admitted.
+
+Theorem skipn_1_eq_tl : forall (A : Type)(ls : list A),
+  skipn 1 ls = List.tl ls.
+
+  intros.
+  destruct ls; trivial.
+
+Qed.
+
+Theorem Forall2_tl : forall (A B : Type)(P : A -> B -> Prop) ls1 ls2,
+  List.Forall2 P ls1 ls2 ->
+  List.Forall2 P (List.tl ls1) (List.tl ls2).
+
+  intros.
+  inversion H; clear H; subst;
+  simpl.
+  econstructor.
+  trivial.
+
+Qed.
+
+Theorem Forall2_rev : forall (A B : Type)(P : A -> B -> Prop) ls1 ls2,
+  List.Forall2 P ls1 ls2 ->
+  List.Forall2 P (List.rev ls1) (List.rev ls2).
+
+  induction 1; intros; simpl in *.
+  econstructor.
+  eapply Forall2_app.
+  eauto.
+  econstructor.
+  trivial.  
+  econstructor.
+
+Qed.
+
+Theorem bvToNat_Z_to_nat_equiv : forall n x z,
+  (0 <= z)%Z ->
+  sbvToInt n x = z ->
+  bvToNat n x = Z.to_nat z.
+
+Admitted.
+
+Theorem bvSShr_Z_shiftr_equiv : forall n x1 x2 y1 y2,
+  Z.of_nat y1 = y2 ->
+  sbvToInt _ x1 = x2 ->
+  sbvToInt _ (bvSShr n x1 y1) = Z.shiftr x2 y2.
+Admitted.
+
 
 
