SAW/spec/EC/Coq/ECEqProof.v
@@ -29,6 +29,8 @@ From Crypto Require Import Algebra.Field.
 From Crypto Require Import Algebra.Nsatz.
 
 From Crypto Require Import Curves.Weierstrass.Jacobian.
+From Crypto Require Import Curves.Weierstrass.Affine.
+From Crypto Require Import Curves.Weierstrass.AffineProofs.
 
 
 From Top Require Import GroupMulWNAF.
@@ -38,103 +40,6 @@ From Top Require Import EC_fiat_P384_gen.
 From Top Require Import CryptoToCoq_equiv.
 
 Set Implicit Arguments.
-
-Theorem bvToNat_toZ_equiv : forall n x,
-  (BinInt.Z.of_nat (bvToNat n x)) = bvToInt n x.
-Admitted.
-
-Theorem sbvToInt_bvToInt_id : forall n x,
-  intToBv n (sbvToInt n x) = x.
-Admitted.
-
-Theorem ecEq_bv_true : forall n v,  
-  ecEq (bitvector n) (PEqWord n) v v = true.
-
-  intros.
-  apply bvEq_refl.
-
-Qed.
-
-Theorem ecEq_bv_false : forall n v1 v2,
-  v1 <> v2 ->
-  ecEq (bitvector n) (PEqWord n) v1 v2 = false.
-
-  intros.
-  unfold ecEq.
-  simpl.
-  case_eq (bvEq n v1 v2); intros; trivial.
-  apply bvEq_eq in H0.
-  intuition.
-Qed.
-
-Theorem ecEq_vec_bv_true : forall n1 n2 v,
-  (ecEq (Vec n1 (bitvector n2)) (PEqVec n1 (bitvector n2) (PEqWord n2)) v v) = true.
-
-  intros.
-  unfold ecEq.
-  simpl.
-  unfold vecEq.
-  Locate foldr.
-  Print foldr.
-
-  Print SAWCoreVectorsAsCoqVectors.
-
-Admitted.
-
-Theorem ecEq_vec_bv_false : forall n1 n2 v1 v2,
-  v1 <> v2 ->
-  (ecEq (Vec n1 (bitvector n2)) (PEqVec n1 (bitvector n2) (PEqWord n2)) v1 v2) = false.
-
-Admitted.
-
-Theorem ecNotEq_vec_bv_false : forall n1 n2 v,
-  (ecNotEq (Vec n1 (bitvector n2)) (PEqVec n1 (bitvector n2) (PEqWord n2)) v v) = false.
-
-    intros.
-  unfold ecNotEq.
-  
-
-Admitted.
-
-Theorem ecNotEq_vec_bv_true : forall n1 n2 v1 v2,
-  v1 <> v2 ->
-  (ecNotEq (Vec n1 (bitvector n2)) (PEqVec n1 (bitvector n2) (PEqWord n2)) v1 v2) = true.
-Admitted.
-
-Theorem rep_false_eq_int_bv : forall n, (replicate n _ false) = (intToBv n 0).
-
-Admitted.
-
-Theorem ecOr_0_if : forall n x y, 
-    ecOr (bitvector n) (PLogicWord n) x y = (replicate n _ false) ->
-    (x = (replicate n _ false) /\ y = (replicate n _ false)).
-Admitted.
-
-Theorem fold_or_impl_0 : forall (n1 n2 : nat) x y,
-  ecFoldl n1 (seq n2 Bool) (seq n2 Bool) (ecOr (seq n2 Bool) (PLogicSeqBool n2))
-     y x = intToBv n2 0 ->
-  (x = (replicate n1 _ (replicate n2 _ false)) /\ y = (replicate n2 _ false)).
-
-  induction n1; intros; simpl in *.
-  unfold replicate. simpl in *.
-  generalize H.
-  eapply (case0 (fun x => foldl (bitvector n2) (bitvector n2) 0%nat (ecOr (bitvector n2) (PLogicWord n2)) y x = intToBv n2 0 ->
-x = nil (Vec n2 bool) /\ y = gen n2 bool (fun _ : Nat => false))); eauto; intuition.
-  simpl in *; subst.
-  rewrite <- rep_false_eq_int_bv.
-  trivial.
-
-  unfold replicate in *. simpl.
-  generalize H.
-  eapply (caseS' x); intuition;
-  simpl in *;
-  edestruct IHn1; eauto;
-  subst.
-  f_equal.
-  edestruct ecOr_0_if; eauto.
-  edestruct ecOr_0_if; eauto.
-
-Qed.
 
 Require Import CryptolToCoq.SAWCoreVectorsAsCoqVectors.
 
@@ -148,12 +53,14 @@ Section ECEqProof.
   Variable Fadd  : F -> F -> F.
   Variable Fsub  : F -> F -> F.
   Variable Fmul  : F -> F -> F.
-  Variable Fsquare : F -> F.
+  (* Variable Fsquare : F -> F. *)
   Variable Finv : F -> F.
   Definition Fdiv (x y:F) := Fmul x (Finv y).
 
+(*
   Variable fiat_from_bytes : seq 384 Bool -> F.
   Variable fiat_to_bytes : F -> seq 384 Bool.
+*)
 
   Local Notation "0" := Fzero.  Local Notation "1" := Fone.
   Local Infix "+" := Fadd. Local Infix "-" := Fsub.
@@ -189,8 +96,19 @@ Section ECEqProof.
   Hypothesis Feq_dec : DecidableRel (@eq F).
   Existing Instance Feq_dec.
 
-  (* Here we assume the field has characteristic at least 3. *)
-  Hypothesis Fchar_3 : @Ring.char_ge F (@eq F) Fzero Fone Fopp Fadd Fsub Fmul 3.
+  (* Here we assume the field has characteristic at least 12. *)
+  (* This is necessary for the base point to generate a group. *)
+  Hypothesis Fchar_12 : @Ring.char_ge F (@eq F) Fzero Fone Fopp Fadd Fsub Fmul 12.
+  Existing Instance Fchar_12.
+
+  (* Point addition requires the field to have characteristic at least 3. *)
+  Theorem Fchar_3 : @Ring.char_ge F (@eq F) Fzero Fone Fopp Fadd Fsub Fmul 3.
+
+    eapply char_ge_weaken.
+    eauto.
+    lia.
+
+  Qed.
   Existing Instance Fchar_3.
 
   Lemma zero_squared_zero : 0^2 = 0.
@@ -234,9 +152,6 @@ Section ECEqProof.
   Definition fromPoint (p:point) : (F*F*F) :=
     proj1_sig p.
 
-  Definition fiat_point_add := fiat_point_add Fsquare Fmul Fsub Fadd.
-  Definition fiat_point_add_jac := fiat_point_add false.
-
   Definition prodToSeq(p : F * F * F) : seq 3 F :=
     cons _ (fst (fst p)) _ (cons _ (snd (fst p)) _ (cons _ (snd p) _ (@nil F))).
 
@@ -254,11 +169,6 @@ Section ECEqProof.
 
   Definition seqToProd(p : seq 3 F) : F * F * F :=
     (nth_order p zero_lt_three, nth_order p one_lt_three, nth_order p two_lt_three).
-
-  Definition fiat_point_add_jac_prod (p1 p2 : (F * F * F)) : (F * F * F) :=
-    let p3 := fiat_point_add_jac (prodToSeq p1) (prodToSeq p2) in
-    (seqToProd p3).
-
 
   Definition is_jacobian (p : F * F * F) :=
     let '(X, Y, Z) := p in
@@ -291,20 +201,254 @@ Section ECEqProof.
   Definition zero_point : point :=
     exist _ zero_point_h zero_point_is_jacobian.
 
+  Definition toPoint(p : F * F * F)(pf : is_jacobian p) : point :=
+    exist _ p pf.
+
+  
+  Definition jac_eq (p1 p2 : F * F * F) :=
+    let '(X1, Y1, Z1) := p1 in
+    let '(X2, Y2, Z2) := p2 in
+      if dec (Feq Z1 Fzero)
+      then Feq Z2 Fzero
+      else
+       ~ Feq Z2 Fzero /\
+       Feq (Fmul X1 (Fmul Z2 Z2)) (Fmul X2 (Fmul Z1 Z1)) /\
+       Feq (Fmul Y1 (Fmul (Fmul Z2 Z2) Z2)) (Fmul Y2 (Fmul (Fmul Z1 Z1) Z1)).
+
+  Theorem jac_eq_refl : forall p, jac_eq p p.
+
+    intros.
+    unfold jac_eq.
+    destruct p.
+    destruct p.
+    destruct (dec (Feq f 0)).
+    trivial.
+    intuition idtac.
+    reflexivity.
+    reflexivity.
+  Qed.
+
+
+  Theorem jac_eq_refl_gen : forall p1 p2,
+    p1 = p2 ->
+    jac_eq p1 p2.
+
+    intros.
+    rewrite H.
+    apply jac_eq_refl.
+
+  Qed.
+
+  Theorem fmul_same_r : forall x v1 v2,
+    Feq v1 v2 ->
+    Feq (v1 * x) (v2 * x).
+
+    intros.
+    rewrite H.
+    reflexivity.
+  Qed.
+
+  Theorem fadd_same_r : forall x v1 v2,
+    Feq v1 v2 ->
+    Feq (v1 + x) (v2 + x).
+
+    intros.
+    rewrite H.
+    reflexivity.
+  Qed.
+
+  Theorem f_zero_absorb : forall (x : F),
+    Feq (x * 0) 0.
+
+    intros.
+    symmetry.
+    rewrite <- (right_identity (x * 0)).
+    rewrite <- (right_inverse (x * 0)) at 1.
+    rewrite <- (right_inverse (x * 0)) at 4.
+    rewrite (associative (x * 0)).
+    apply fadd_same_r.
+    rewrite <- left_distributive.
+    rewrite right_identity.
+    reflexivity.
+
+  Qed.
+
+  Theorem square_nz : forall (x : F),
+    x <> 0 ->
+    x ^ 2 <> 0.
+
+    intuition idtac.
+    eapply (@fmul_same_r (Finv x)) in H0.
+    rewrite <- (associative x) in H0.
+    rewrite (commutative _ (Finv x)) in H0.
+    rewrite left_multiplicative_inverse in H0.
+    rewrite right_identity in H0.
+    rewrite (commutative 0) in H0.
+    rewrite f_zero_absorb in H0.
+    intuition idtac.
+    intuition idtac.
+
+  Qed.
+
+  Theorem cube_nz : forall (x : F),
+    x <> 0 ->
+    x ^ 3 <> 0.
+
+    intuition idtac.
+    eapply (@fmul_same_r (Finv x)) in H0.
+    rewrite <- (associative x) in H0.
+    rewrite (commutative _ (Finv x)) in H0.
+    rewrite (associative (Finv x)) in H0.
+    rewrite left_multiplicative_inverse in H0.
+    rewrite left_identity in H0.
+    rewrite (commutative 0) in H0.
+    rewrite f_zero_absorb in H0.
+
+    eapply (@fmul_same_r (Finv x)) in H0.
+    rewrite <- (associative x) in H0.
+    rewrite (commutative _ (Finv x)) in H0.
+    rewrite left_multiplicative_inverse in H0.
+    rewrite right_identity in H0.
+    rewrite (commutative 0) in H0.
+    rewrite f_zero_absorb in H0.
+    intuition idtac.
+    intuition idtac.
+    intuition idtac.
+
+  Qed.
+
+  Theorem jac_eq_trans : forall p1 p2 p3,
+    jac_eq p1 p2 ->
+    jac_eq p2 p3 ->
+    jac_eq p1 p3.
+
+    intros.
+    unfold jac_eq in *.
+    destruct p1. destruct p. destruct p2. destruct p.
+    destruct p3. destruct p.
+    destruct (dec (Feq f 0)).
+    destruct (dec (Feq f2 0));
+    intuition idtac.
+    destruct (dec (Feq f2 0)); intuition idtac.
+
+    eapply (@fmul_same_r (Finv (f^2))) in H0.
+    rewrite <- (associative f3) in H0.
+    rewrite (commutative (f^2)) in H0.
+    rewrite left_multiplicative_inverse in H0.
+    rewrite right_identity in H0.
+    rewrite <- H0 in H2.
+    eapply (@fmul_same_r (Finv (f2^2))) in H2.
+    rewrite <- (associative f6) in H2.
+    rewrite (commutative (f2^2)) in H2.
+    rewrite left_multiplicative_inverse in H2.
+    rewrite right_identity in H2.
+    rewrite (commutative _ (Finv (f2^2))) in H2.
+    rewrite (commutative f0) in H2.
+    do 3 rewrite (associative (Finv (f2^2))) in H2.    
+    rewrite left_multiplicative_inverse in H2.
+    rewrite left_identity in H2.
+    eapply (@fmul_same_r (f^2)) in H2.
+    rewrite (commutative _ (f^2)) in H2.
+    rewrite (commutative f0) in H2.
+    do 2 rewrite (associative (f^2)) in H2.
+    rewrite (commutative (f^2)) in H2.
+    rewrite left_multiplicative_inverse in H2.
+    rewrite left_identity in H2.
+    trivial.
+
+    eauto using square_nz.
+    eauto using square_nz.
+    eauto using square_nz.
+    eauto using square_nz.  
+    
+    eapply (@fmul_same_r (Finv (f^3))) in H4.
+    rewrite <- (associative f4) in H4.
+    rewrite (commutative (f^3)) in H4.
+    rewrite left_multiplicative_inverse in H4.
+    rewrite right_identity in H4.
+    rewrite <- H4 in H5.
+    eapply (@fmul_same_r (Finv (f2^3))) in H5.
+    rewrite <- (associative f7) in H5.
+    rewrite (commutative (f2^3)) in H5.
+    rewrite left_multiplicative_inverse in H5.
+    rewrite right_identity in H5.
+    rewrite (commutative _ (Finv (f2^3))) in H5.
+    rewrite (commutative f1) in H5.
+    do 3 rewrite (associative (Finv (f2^3))) in H5.    
+    rewrite left_multiplicative_inverse in H5.
+    rewrite left_identity in H5.
+    eapply (@fmul_same_r (f^3)) in H5.
+    rewrite (commutative _ (f^3)) in H5.
+    rewrite (commutative f1) in H5.
+    do 2 rewrite (associative (f^3)) in H5.
+    rewrite (commutative (f^3)) in H5.
+    rewrite left_multiplicative_inverse in H5.
+    rewrite left_identity in H5.
+    trivial.
+    
+    eauto using cube_nz.
+    eauto using cube_nz.
+    eauto using cube_nz.
+    eauto using cube_nz.
+
+  Qed.
+
+  
+  Theorem jac_eq_symm : forall p1 p2,
+    jac_eq p1 p2 ->
+    jac_eq p2 p1.
+
+    intros. 
+    unfold jac_eq in *.
+    destruct p1. destruct p.
+    destruct p2. destruct p.
+    destruct (dec (Feq f 0)).
+    destruct (dec (Feq f2 0));
+    intuition idtac.
+    destruct (dec (Feq f2 0)); 
+    intuition idtac.
+    symmetry.
+    trivial.
+    symmetry.
+    trivial.
+  Qed.
+
+  Theorem jacobian_eq_jac_eq : forall p1 p2,
+    Jacobian.eq p1 p2 ->
+    jac_eq (fromPoint p1) (fromPoint p2).
+
+    intros.
+    unfold jac_eq, fromPoint, Jacobian.eq in *.
+    apply H.
+
+  Qed.
+
+  Variable Fsquare : F -> F.
+
+  Definition fiat_point_add := fiat_point_add Fsquare Fmul Fsub Fadd.
+  Definition fiat_point_add_jac := fiat_point_add false.
+
+  Definition fiat_point_add_jac_prod (p1 p2 : (F * F * F)) : (F * F * F) :=
+    let p3 := fiat_point_add_jac (prodToSeq p1) (prodToSeq p2) in
+    (seqToProd p3).
+
+
+(*
   Theorem fiat_point_add_jac_prod_is_jacobian : forall p1 p2,
     is_jacobian p1 ->
     is_jacobian p2 ->
     is_jacobian (fiat_point_add_jac_prod p1 p2).
-  Admitted.
 
-  Definition toPoint(p : F * F * F)(pf : is_jacobian p) : point :=
-    exist _ p pf.
+    intros.
+    unfold is_jacobian, fiat_point_add_jac_prod, fiat_point_add_jac in *.
+    
+  Qed.
 
   Definition fiat_point_add_jacobian (p1 p2 : point) : point :=
     toPoint 
       (fiat_point_add_jac_prod (fromPoint p1) (fromPoint p2)) 
       (fiat_point_add_jac_prod_is_jacobian (fromPoint p1) (fromPoint p2) (proj2_sig p1) (proj2_sig p2)).
-
+*)
 
   (* Assume that squaring satisifes its spec. *)
   Hypothesis fiat_field_square_spec : forall (x : F), Fsquare x = Fmul x x.
@@ -338,16 +482,32 @@ Section ECEqProof.
 
   Theorem prodToSeq_inv : forall x, prodToSeq (seqToProd x) = x.
 
-  Admitted.
+    intros.
+    unfold seqToProd, prodToSeq.
+    simpl.
+    destruct (Vec_S_cons x).
+    destruct H.
+    destruct (Vec_S_cons x1).
+    destruct H0.
+    destruct (Vec_S_cons x3).
+    destruct H1.
+    subst.
+    rewrite (Vec_0_nil x5).
+    reflexivity.
+  Qed.
 
   Theorem seqToProd_inv : forall x, seqToProd (prodToSeq x) = x.
-
-  Admitted.
+    intros.
+    unfold seqToProd, prodToSeq.
+    simpl.
+    destruct x.
+    destruct p.
+    reflexivity.
+  Qed.
 
   Theorem double_eq_minus_3 : forall p:point,
       prodToSeq (fromPoint (Jacobian.double_minus_3 a_is_minus_3 p)) =
       (fiat_point_double (prodToSeq (fromPoint p))).
-  Proof.
 
     intros.
     rewrite double_eq_minus_3_h.
@@ -356,47 +516,7 @@ Section ECEqProof.
 
   Qed.
 
-  Definition jac_eq (p1 p2 : F * F * F) :=
-    let '(X1, Y1, Z1) := p1 in
-    let '(X2, Y2, Z2) := p2 in
-      if dec (Feq Z1 Fzero)
-      then Feq Z2 Fzero
-      else
-       ~ Feq Z2 Fzero /\
-       Feq (Fmul X1 (Fmul Z2 Z2)) (Fmul X2 (Fmul Z1 Z1)) /\
-       Feq (Fmul Y1 (Fmul (Fmul Z2 Z2) Z2)) (Fmul Y2 (Fmul (Fmul Z1 Z1) Z1)).
-
-  Theorem jac_eq_refl : forall p, jac_eq p p.
-  Admitted.
-
-
-  Theorem jac_eq_refl_gen : forall p1 p2,
-    p1 = p2 ->
-    jac_eq p1 p2.
-
-    intros.
-    rewrite H.
-    apply jac_eq_refl.
-
-  Qed.
-
-  Theorem jac_eq_trans : forall p1 p2 p3,
-    jac_eq p1 p2 ->
-    jac_eq p2 p3 ->
-    jac_eq p1 p3.
-  Admitted.
-
-  Theorem jac_eq_symm : forall p1 p2,
-    jac_eq p1 p2 ->
-    jac_eq p2 p1.
-  Admitted.
-
-  Theorem jacobian_eq_jac_eq : forall p1 p2,
-    Jacobian.eq p1 p2 ->
-    jac_eq (fromPoint p1) (fromPoint p2).
-  Admitted.
-
-  Lemma point_add_jac_eq_old : forall (a b:point),
+  Lemma point_add_jac_eq_h : forall (a b:point),
       jac_eq (fromPoint (Jacobian.add a b))
       (seqToProd (fiat_point_add_jac (prodToSeq (fromPoint a)) (prodToSeq (fromPoint b)))).
   Proof.
@@ -477,76 +597,549 @@ Section ECEqProof.
 
   Qed.
 
+  Theorem square_mul_eq : forall (x y : F),
+    (x * y)^2 = x^2 * y^2.
+  
+    intros.
+    repeat rewrite associative.
+    f_equal.
+    rewrite <- (associative x x).  
+    rewrite <- associative.
+    f_equal.
+    apply commutative.
+  Qed.
+
+  Theorem cube_mul_eq : forall (x y : F),
+    (x * y)^3 = x^3 * y^3.
+
+    intros.
+    rewrite square_mul_eq.
+    repeat rewrite <- (associative (x^2)).
+    f_equal.
+    rewrite (commutative x (y^3)).
+    rewrite <- (associative (y^2)).
+    f_equal.
+    apply commutative.
+  Qed.
+
+
+  Theorem jac_eq_jacobian_eq:
+    forall p1 p2 : Jacobian.point,
+    jac_eq (fromPoint p1) (fromPoint p2) -> Jacobian.eq p1 p2.
+
+    intros.
+    eauto.
+
+  Qed.
+
+  Theorem fmul_same_r_if : forall (x y z : F),
+    ~ (Feq x 0) ->
+    Feq (y * x) (z * x) ->
+    Feq y z.
+
+    intros.
+    eapply (fmul_same_r (Finv x)) in H0.
+    rewrite <- associative in H0.
+    rewrite (commutative x) in H0.
+    rewrite left_multiplicative_inverse in H0.
+    rewrite right_identity in H0.
+    rewrite <- associative in H0.
+    rewrite (commutative x) in H0.
+    rewrite left_multiplicative_inverse in H0.
+    rewrite right_identity in H0.
+    trivial.
+    trivial.
+    trivial.
+
+  Qed.
+
+  Theorem fadd_same_r_if : forall (x y z : F),
+    Feq (y + x) (z + x) ->
+    Feq y z.
+
+    intros.
+    eapply (fadd_same_r (Fopp x)) in H.
+    rewrite <- associative in H.
+    rewrite (commutative x) in H.
+    rewrite left_inverse in H.
+    rewrite right_identity in H.
+    rewrite <- associative in H.
+    rewrite (commutative x) in H.
+    rewrite left_inverse in H.
+    rewrite right_identity in H.
+    trivial.
+
+  Qed.
+
+  Theorem mul_nz : forall (x y : F),
+    ~(Feq x 0) ->
+    ~(Feq y 0) ->
+    ~(Feq (x * y) 0).
+
+    intuition idtac.
+    
+    eapply (@fmul_same_r (Finv y)) in H1.
+    rewrite <- (associative x) in H1.
+    rewrite (commutative _ (Finv y)) in H1.
+    rewrite left_multiplicative_inverse in H1.
+    rewrite right_identity in H1.
+    rewrite (commutative 0) in H1.
+    rewrite f_zero_absorb in H1.
+    intuition idtac.
+    intuition idtac.
+
+  Qed.
+
+  Theorem inv_mul_eq : forall (x y : F),
+    ~(Feq y 0) ->
+    ~(Feq x 0) ->
+    Finv (x*y) = ((Finv x) * (Finv y)).
+
+    intros.
+    eapply (@fmul_same_r_if y).
+    trivial.
+    rewrite <- associative.
+    rewrite left_multiplicative_inverse; trivial.
+    rewrite right_identity.
+    
+    eapply (@fmul_same_r_if x).
+    trivial.
+    rewrite left_multiplicative_inverse; trivial.
+    rewrite <- associative.
+    rewrite (commutative y).
+    apply left_multiplicative_inverse.
+    apply mul_nz; eauto.
+ 
+  Qed.
+
+  Theorem inv_square_eq : forall (x : F),
+    ~(Feq x 0) ->
+    (Finv x)^2 = Finv (x^2).
+
+    symmetry.
+    apply inv_mul_eq; eauto.
+
+  Qed.
+
+  Theorem inv_cube_eq : forall (x : F),
+    ~(Feq x 0) ->
+    (Finv x)^3 = Finv (x^3).
+
+    symmetry.
+    rewrite inv_mul_eq; eauto.
+    rewrite inv_square_eq; eauto.
+    apply square_nz; trivial.
+
+  Qed.
+
+  Theorem fromPoint_is_jacobian : forall p,
+    is_jacobian (fromPoint p).
+
+    intros.
+    unfold is_jacobian, fromPoint.
+    destruct p.
+    simpl.
+    trivial.
+  Qed.
+
+  Theorem cube_square_eq : forall (x : F),
+    ((x^3)^2) = ((x^2)^3).
+
+    intros.
+    repeat rewrite associative.
+    reflexivity.
+
+  Qed.
+
+  Theorem jac_eq_is_jacobian : forall p1 p2,
+    is_jacobian p1 ->
+    jac_eq p1 p2 ->
+    is_jacobian p2.
+
+    intros.
+    unfold is_jacobian, jac_eq in *.
+    destruct p1. destruct p.
+    destruct p2. destruct p.
+    destruct (dec (Feq f2 0)).
+    trivial.
+
+    destruct (dec (Feq f 0)).
+    intuition idtac.
+    intuition idtac.
+
+    apply (fmul_same_r (Finv (f2^2))) in H0.
+    rewrite <- associative in H0.
+    rewrite (commutative (f2^2) (Finv (f2^2))) in H0.
+    rewrite left_multiplicative_inverse in H0.
+    rewrite right_identity in H0.
+
+    apply (fmul_same_r (Finv (f2^3))) in H3.
+    rewrite <- associative in H3.
+    rewrite (commutative (f2^3) (Finv (f2^3))) in H3.
+    rewrite left_multiplicative_inverse in H3.
+    rewrite right_identity in H3.
+
+    rewrite H0 in H.
+    rewrite H3 in H.
+    repeat rewrite cube_mul_eq in *.
+    repeat rewrite square_mul_eq in *.
+
+    apply (fmul_same_r (Finv ((f^2)^3))) in H.
+    rewrite (commutative (f4^2) ((f^2)^3)) in H.
+    rewrite (commutative _ (Finv _)) in H.
+    do 2 rewrite (associative (Finv ((f ^ 2) ^ 3))) in H.
+    rewrite left_multiplicative_inverse in H.
+    rewrite left_identity in H.
+    repeat rewrite right_distributive in H.
+    rewrite (commutative _ (Finv ((f^2)^3))) in H.
+    rewrite (commutative (f3^3)) in H.
+    do 2 rewrite (associative (Finv ((f ^ 2) ^ 3))) in H.
+    rewrite left_multiplicative_inverse in H.
+    rewrite left_identity in H.
+    rewrite <- (associative b) in H.
+    rewrite (commutative ((f^2)^3)) in H.
+    rewrite left_multiplicative_inverse in H.
+    rewrite right_identity in H.
+    replace (a * (f3 * f ^ 2 * Finv (f2 ^ 2)) * (f ^ 2) ^ 2 * Finv ((f ^ 2) ^ 3))
+        with (a * (f3 * Finv (f2 ^ 2)))
+        in H.
+    apply (fmul_same_r ((f2^3)^2)) in H.
+    rewrite <- (associative) in H.
+    rewrite inv_square_eq in H.
+    rewrite left_multiplicative_inverse in H.
+    rewrite right_identity in H.
+    rewrite H.
+    repeat rewrite right_distributive.
+    rewrite <- (associative (f3^3)).
+    repeat rewrite inv_cube_eq.
+    repeat rewrite cube_square_eq.
+    rewrite left_multiplicative_inverse.
+    rewrite right_identity.
+    apply fadd_same_r.
+    repeat rewrite (commutative (f3^3)).
+    apply fadd_same_r.
+    repeat rewrite <- (associative a).
+    repeat rewrite (commutative a).
+    apply fmul_same_r.
+    rewrite <- (associative f3).
+    repeat rewrite (commutative f3).
+    apply fmul_same_r.
+    replace ((f2^2)^3) with ((f2^2) * ((f2^2)^2)).
+    rewrite (associative (Finv (f2^2))).
+    rewrite left_multiplicative_inverse.
+    rewrite left_identity.
+    reflexivity.
+    apply square_nz; trivial.
+    repeat rewrite associative.
+    reflexivity.
+    eauto using square_nz, cube_nz.
+    eauto using square_nz, cube_nz.
+    eauto using square_nz, cube_nz.
+    eauto using square_nz, cube_nz.
+
+    repeat rewrite <- (associative a).
+    repeat rewrite (commutative a).
+    apply fmul_same_r.
+    repeat rewrite <- (associative f3).
+    repeat rewrite (commutative f3).
+    apply fmul_same_r.
+    rewrite (commutative (f^2)).
+    repeat rewrite <- (associative (Finv (f2^2))).
+    replace (f ^ 2 * (f ^ 2) ^ 2) with ((f ^ 2) ^ 3).
+    rewrite (commutative ((f^2)^3)).
+    rewrite left_multiplicative_inverse.
+    rewrite right_identity.
+    reflexivity.
+    eauto using square_nz, cube_nz.
+    repeat rewrite associative.
+    reflexivity.
+
+    eauto using square_nz, cube_nz.
+    eauto using square_nz, cube_nz.
+    eauto using square_nz, cube_nz.
+    eauto using square_nz, cube_nz.
+    eauto using square_nz, cube_nz.
+
+  Qed.
+
+  Theorem fromPoint_toPoint_id : forall p (H : is_jacobian p),
+    p = fromPoint (toPoint _ H).
+  
+    intros.
+    reflexivity.
+  Qed.
+
+  Theorem jac_eq_point_ex : forall p1 p2,
+    jac_eq (fromPoint p1) p2 ->
+    exists p2', p2 = fromPoint p2'.
+
+    intros.
+    Search is_jacobian.
+    assert (is_jacobian p2).
+    eapply jac_eq_is_jacobian; eauto.
+    apply fromPoint_is_jacobian.
+    exists (toPoint _ H0).
+    reflexivity.
+  Qed.
+
+
+ 
   (* Need a more general form of the point add correctness proof using Jacobian equality *)
   Lemma point_add_jac_eq : forall (a b:point) a' b',
     jac_eq (fromPoint a) (seqToProd a') ->
     jac_eq (fromPoint b) (seqToProd b') -> 
     jac_eq (fromPoint (Jacobian.add a b)) (seqToProd (fiat_point_add_jac a' b')).
 
-  Admitted.
+    intros.  
+    edestruct (jac_eq_point_ex _ _ H).
+    edestruct (jac_eq_point_ex _ _ H0).
+    
+    eapply jac_eq_trans.
+    eapply jacobian_eq_jac_eq.
+    eapply Jacobian.Proper_add.
+    eapply jac_eq_jacobian_eq.
+    rewrite H1 in H.
+    eauto.
+    eapply jac_eq_jacobian_eq.
+    rewrite H2 in H0.
+    eauto.
+    eapply jac_eq_trans.
+    eapply point_add_jac_eq_h.
+    rewrite <- H1.
+    rewrite <- H2.
+    repeat rewrite prodToSeq_inv.
+    apply jac_eq_refl.
+ 
+  Qed.
 
   Definition groupMul := @groupMul point Jacobian.add zero_point.
   Definition fiat_point_mul := fiat_point_mul Fsquare Fmul Fsub Fadd Fopp.
 
-  Variable min_l : forall n, Nat.min n n = n.
+  (* Variable min_l : forall n, Nat.min n n = n.*)
 
   (* Jacobian.v defines an Equivalence instance for Jacobian.eq. Use this to construct a Setoid. *)
   Instance jac_eq_setoid : Setoid point := {equiv := Jacobian.eq}.
 
-  Theorem jac_add_assoc : forall (a b c : point),
-    (Jacobian.add (Jacobian.add a b) c) == (Jacobian.add a (Jacobian.add b c)).
+  Theorem jac_eq_from_affine : forall (x y : point),
+    WeierstrassCurve.W.eq (Jacobian.to_affine x) (Jacobian.to_affine y) ->
+    x == y.
+  
+    intros.
+    rewrite <- Jacobian.of_affine_to_affine.
+    symmetry.
+    rewrite <- Jacobian.of_affine_to_affine.
+    symmetry.
+    apply Jacobian.Proper_of_affine.
+    trivial.
+  Qed.
 
-  Admitted.
+  Definition wpoint := @WeierstrassCurve.W.point F Feq Fadd Fmul a b.
+
+  Definition W_opp : wpoint -> wpoint := W.opp.
+
+  (* Discriminant is non-zero *)
+  (* Can we simplify this assumption because a=-3 *)
+  Hypothesis discriminant_nonzero : 
+    ~
+Feq
+  ((1 + 1 + 1 + 1) * a * a * a +
+   ((1 + 1 + 1 + 1) ^ 2 + (1 + 1 + 1 + 1) + (1 + 1 + 1 + 1) + 1 + 1 + 1) * b * b) 0.
+
+  Instance W_commutative_group : 
+    @commutative_group wpoint
+    WeierstrassCurve.W.eq
+    WeierstrassCurve.W.add
+    WeierstrassCurve.W.zero
+    W.opp.
+
+    apply W.commutative_group.
+    apply Fchar_12.
+    unfold Datatypes.id.
+    trivial.
+
+  Defined.
+
+
+  Theorem jac_add_assoc : forall (x y z : point),
+    (Jacobian.add (Jacobian.add x y) z) == (Jacobian.add x (Jacobian.add y z)).
+
+    intros.
+    apply jac_eq_from_affine.
+
+    repeat rewrite Jacobian.to_affine_add.
+    rewrite associative.
+    reflexivity.
+
+  Qed.
 
   Theorem jac_add_comm : forall (a b : point),
     (Jacobian.add a b) == (Jacobian.add b a).
 
-  Admitted.
+    intros.
+    apply jac_eq_from_affine.
+    repeat rewrite Jacobian.to_affine_add.
+    apply commutative.
+
+  Qed.
+
+  Theorem to_affine_zero : WeierstrassCurve.W.eq (Jacobian.to_affine zero_point) WeierstrassCurve.W.zero.
+
+    unfold WeierstrassCurve.W.eq, Jacobian.to_affine, zero_point.
+    simpl.
+    destruct (dec (Feq 0 0)); trivial.
+    intuition idtac.
+    eapply n.
+    reflexivity.
+  Qed.
 
   Theorem jac_add_id_l : forall (a : point),
     (Jacobian.add zero_point a) == a.
-  Admitted.
+
+    intros.
+    apply jac_eq_from_affine.
+    repeat rewrite Jacobian.to_affine_add.
+    rewrite to_affine_zero.  
+    apply left_identity.
+
+  Qed.
 
   Theorem jac_double_correct : forall (a : point),
     (Jacobian.double a) == (Jacobian.add a a).
-  Admitted.
+
+    intros.
+    apply jac_eq_from_affine.
+    rewrite Jacobian.to_affine_add.
+    rewrite Jacobian.to_affine_double.
+    reflexivity.
+
+  Qed.
+
+  Theorem opp_mul_eq : forall (x : F),
+    Feq (Fopp x) ((Fopp 1) * x).
+
+    intros.
+    eapply (@fadd_same_r_if x).
+    rewrite left_inverse.
+    replace x with (1 * x) at 2.
+    rewrite <- right_distributive.
+    rewrite left_inverse.
+    symmetry.
+    rewrite commutative.
+    apply f_zero_absorb.
+    apply left_identity.
+
+  Qed.
+
+  Theorem to_affine_opp : forall x, 
+    WeierstrassCurve.W.eq (Jacobian.to_affine (Jacobian.opp x)) (W_opp (Jacobian.to_affine x)).
+
+    intros.
+
+    unfold WeierstrassCurve.W.eq, Jacobian.to_affine, Jacobian.opp, W_opp.
+    simpl.
+    destruct x.
+    simpl.
+    destruct x.
+    destruct p.
+    destruct (dec (Feq f 0)); intuition idtac.
+    reflexivity.
+    repeat rewrite field_div_definition.
+    rewrite (@opp_mul_eq (f1 * Finv (f ^ 3))).
+    rewrite (opp_mul_eq).
+    symmetry.
+    apply associative.
+  Qed.
 
   Theorem jac_opp_correct : forall (a : point),
     (Jacobian.add a (Jacobian.opp a)) == zero_point.
-  Admitted.
+
+    intros.
+    apply jac_eq_from_affine.
+    rewrite Jacobian.to_affine_add.
+    rewrite to_affine_zero.
+    rewrite to_affine_opp.
+    apply right_inverse.
+  Qed.
+
+  Definition wzero : wpoint := WeierstrassCurve.W.zero.
+
+  Theorem w_add_same_r : forall (z x y : wpoint),
+    WeierstrassCurve.W.eq x y ->
+    WeierstrassCurve.W.eq (WeierstrassCurve.W.add x z) (WeierstrassCurve.W.add y z).
+
+    intros.
+    rewrite H.
+    reflexivity.
+
+  Qed.
+
+  Theorem w_add_same_r_if : forall (z x y : wpoint),
+    WeierstrassCurve.W.eq (WeierstrassCurve.W.add x z) (WeierstrassCurve.W.add y z) ->
+    WeierstrassCurve.W.eq x y.
+
+    intros.
+    apply (@w_add_same_r (W_opp z)) in H.
+    repeat rewrite <- associative in H.
+    rewrite right_inverse in H.
+    repeat rewrite right_identity in H.
+    trivial.
+  Qed.
+
+
+  Theorem w_opp_add_distr : forall (x y : wpoint),
+    WeierstrassCurve.W.eq (W_opp (WeierstrassCurve.W.add x y)) (WeierstrassCurve.W.add (W_opp x) (W_opp y)).
+
+    intros.
+    eapply (@w_add_same_r_if (WeierstrassCurve.W.add x y)).
+    rewrite left_inverse.
+    rewrite (commutative x).
+    rewrite <- associative.
+    rewrite (associative (W_opp y)).
+    rewrite left_inverse.
+    rewrite left_identity.
+    rewrite left_inverse.
+    reflexivity.
+  Qed.
+
 
   Theorem jac_opp_add_distr : forall (a b : point),
     (Jacobian.opp (Jacobian.add a b)) == (Jacobian.add (Jacobian.opp a) (Jacobian.opp b)).
-  Admitted.
+
+    intros.
+    apply jac_eq_from_affine.
+    repeat rewrite to_affine_opp.
+    repeat rewrite Jacobian.to_affine_add.
+    repeat rewrite to_affine_opp.
+    apply w_opp_add_distr.
+
+  Qed.
+
+  Theorem w_opp_involutive  : forall (x : wpoint),
+    WeierstrassCurve.W.eq (W_opp (W_opp x)) x.
+
+    intros.
+    apply (@w_add_same_r_if (W_opp x)).
+    rewrite left_inverse.
+    rewrite right_inverse.
+    reflexivity.
+
+  Qed.
 
   Theorem jac_opp_involutive  : forall (a : point),
     (Jacobian.opp (Jacobian.opp a)) == a.
-  Admitted.
+
+    intros.
+    intros.
+    apply jac_eq_from_affine.
+    repeat rewrite to_affine_opp.
+    apply w_opp_involutive.
+  Qed.
 
   Definition seqToList(A : Type)(n : nat)(s : seq n A) : list A :=
     to_list s.
 
   Definition windowsSeqToList (n : nat)(s : seq n (seq 16 Bool)) : list SignedWindow := 
     List.map (toSignedInteger 16) (seqToList s).
-
-    (*
-  Definition fiat_pre_comp_table_gen (pred_pred_tsize : nat)
-    (p : CryptolPrimitivesForSAWCore.seq (CryptolPrimitivesForSAWCore.TCNum 3) (CryptolPrimitivesForSAWCore.seq (CryptolPrimitivesForSAWCore.TCNum 6) (CryptolPrimitivesForSAWCore.seq (CryptolPrimitivesForSAWCore.TCNum 64) SAWCoreScaffolding.Bool)))  :=
-   
-(scanl Integer (Vec 3 (Vec 6 (bitvector 64))) (S pred_pred_tsize)
-        (fun (z : Vec 3 (Vec 6 (bitvector 64))) (_ : Integer) =>
-         EC_fiat_P384_7.fiat_point_add Fsquare Fmul Fsub Fadd false
-           (EC_fiat_P384_7.fiat_point_double Fsquare Fmul Fsub Fadd p) z)
-        p (CryptolPrimitivesForSAWCore.ecFromTo (CryptolPrimitivesForSAWCore.TCNum 1%nat) (CryptolPrimitivesForSAWCore.TCNum (S pred_pred_tsize)) SAWCoreScaffolding.Integer PLiteralInteger)).
-
-  Theorem fiat_pre_comp_table_gen_7_equiv : forall (p : seq 3 (seq 6 (seq 64 Bool))),
-    (fiat_pre_comp_table_gen 62 p) = (fiat_pre_comp_table Fsquare Fmul Fsub Fadd p).
-
-    intros.
-    reflexivity.
-
-  Qed.
-  *)
 
   Fixpoint preCompTable_fix (p : point) n prev :=
     match n with
@@ -591,21 +1184,6 @@ Section ECEqProof.
 
   Qed.
 
-  Theorem scanl_gen_equiv : forall A n f1 f2 z1 x,
-    (scanl Integer A n
-           (fun (z : A) (_ : Integer) =>
-            z1 z) x
-           (gen n Integer f1))
-    = 
-    (scanl Integer A n
-           (fun (z : A) (_ : Integer) =>
-            z1 z) x
-           (gen n Integer f2)).
-
-    induction n; intuition; simpl in *.
-    f_equal.
-    apply IHn.
-  Qed.
 
   Theorem preCompTable_fix_equiv : forall pred_pred_tsize p p2 p2',
     jac_eq (fromPoint p2) (seqToProd p2') ->
@@ -650,110 +1228,78 @@ Section ECEqProof.
     
   Qed.
 
-  Fixpoint bv64Nats_h n v :=
-    match n with
-    | 0 => List.nil
-    | S n' => (intToBv 64 (Z.of_nat v)) :: (bv64Nats_h n' (S v))
-    end.
+(*
+  Theorem Z_sub_range_pos_h : forall x y z,
+    (0 <= x ->
+    0 <= y <= x ->
+    0 <= z <= x ->
+    (-x + -x) <= y - z <= x + x)%Z.
 
-  Definition bv64Nats n := bv64Nats_h n 0.
-
-  Theorem gen_nat_seq_eq_h : forall n v,
-    (to_list
-        (gen n (bitvector 64)
-           (fun i : nat => intToBv 64 (Z.of_nat (addNat i v%nat)))))
-    = bv64Nats_h n v.
-
-    induction n; intuition; simpl in *.
-    rewrite to_list_cons.
-    f_equal.
-    rewrite <- IHn.
-    f_equal.  
-    eapply gen_domain_eq.
     intros.
-    rewrite (eqNatAddComm _ (S v)).
-    simpl.
-    rewrite eqNatAddComm.
+    lia.
+
+  Qed.
+
+  Theorem Z_div2_le : forall x,
+    (2 * (Z.div2 x) <= x)%Z.
+
+    intros.
+    destruct (Zeven.Zeven_odd_dec x).
+    rewrite Zeven.Zeven_div2.
+    reflexivity.
+    trivial.
+    rewrite Zeven.Zodd_div2.
+    lia.
     trivial.
   Qed.
+*)
 
-  Theorem gen_nat_seq_eq : forall n,
-    (to_list
-        (gen n (bitvector 64)
-           (fun i : nat => intToBv 64 (Z.of_nat (addNat i 0%nat)))))
-    = bv64Nats n.
+(*
+  Theorem Z_sub_range_le_lt_pos : forall x y z,
+    (0 <= x ->
+    0 <= y < x ->
+    0 <= z < x ->
+    -x <= y - z < x)%Z.
 
     intros.
-    apply gen_nat_seq_eq_h.    
-  Qed.
-
-  Fixpoint nats_h n v :=
-    match n with
-    | 0 => List.nil
-    | S n' => v :: (nats_h n' (S v))
-    end.
-
-  Definition nats n := nats_h n 0.
-
-  Theorem toN_int_excl_length : forall n, 
-    List.length (toN_excl_int n) = n.
-
-    induction n; intuition idtac; simpl in *.
-
-    rewrite app_length.
-    rewrite IHn.
-    simpl.
+    intuition idtac.
+    rewrite <- (Z.opp_involutive (y - z)).
+    eapply (@Z.opp_le_mono _ x).
+    rewrite Z.opp_sub_distr.
+    eapply Z.le_trans.
+    apply Z.add_le_mono_l.
+    apply Z.lt_le_incl.
+    eauto.
+    eapply Z.le_trans.
+    apply Z.add_le_mono_r.
+    apply Z.opp_nonpos_nonneg.
+    trivial.
+    lia.
+    eapply Z.lt_le_trans.
+    apply Z.sub_lt_mono_r.
+    eauto.
+    eapply Z.le_trans.
+    apply Z.sub_le_mono_l.
+    eauto.
     lia.
 
   Qed.
 
-  Theorem toN_int_length : forall n, 
-    List.length (toN_int n) = (S n).
+*)
 
-    intros.
-    unfold toN_int.
-    rewrite app_length.
-    rewrite toN_int_excl_length.
-    simpl.
-    lia.
+  Theorem sbvToInt_shiftR_equiv:
+  forall [n s : nat] x,
+  s >= 0 ->
+  sbvToInt n (shiftR n bool false x s) =
+  BinInt.Z.shiftr (sbvToInt _ x) (BinInt.Z.of_nat s).
 
-  Qed.
+  Admitted.
 
 
-  Theorem scanl_fix_convert : forall (A1 A2 B1 B2: Type)
-    (conva : A2 -> A1)(convb : B2 -> B1)
-    (f1 : A1 -> A1)(f2 : A2 -> A2)
-    (fb1 : A1 -> B1)(fb2 : A2 -> B2)
-    (fc1 : A1 -> B1)(fc2 : A2 -> B2),
-    (forall a, fb1 (conva a) = convb (fb2 a)) ->
-    (forall a, (exists b, a = (f2 b)) -> fc1 (conva a) = convb (fc2 a)) ->
-    (forall a, (exists b, a = (f2 b)) -> f1 (conva a) = conva (f2 a)) ->
-    forall n a1 a2,
-    (exists b, a2 = (f2 b)) ->
-    a1 = (conva a2) ->
-    List.Forall2 (fun b1 b2 => b1 = convb b2)
-    (scanl_fix f1 fb1 fc1 n a1)
-    (scanl_fix f2 fb2 fc2 n a2).
-
-    induction n; intros; simpl in *; subst.
-    econstructor.
-
-    destruct n.
-    econstructor.
-    eauto.
-    econstructor.
-    eauto.
-    econstructor.
-
-    econstructor.
-    eauto.
-    eapply IHn.
-    eauto.
-    eauto.
-
-  Qed.
-
+(*
   Theorem fiat_mul_scalar_rwnaf_odd_loop_body_gen_equiv : forall wsize z,
+    wsize < 15 -> 
+    sbvToInt _ z = bvToInt _ z ->
     recode_rwnaf_odd_scanl_fix_body wsize (bvToInt _ z) =
     (sbvToInt _ 
           (fst (fiat_mul_scalar_rwnaf_odd_loop_body_gen wsize z)),
@@ -762,38 +1308,325 @@ Section ECEqProof.
 
     intros.
     
+    unfold recode_rwnaf_odd_scanl_fix_body, fiat_mul_scalar_rwnaf_odd_loop_body_gen.
+    simpl.
+    f_equal.
+    rewrite sbvToInt_drop_equiv_h.
+    rewrite sbvToInt_bvSub_equiv.
+    f_equal.
+    rewrite sbvToInt_bvURem_equiv.
+    f_equal.
+    rewrite bvMul_2_shiftl_equiv.
+    rewrite shiftL_shiftL.
+    rewrite bvToInt_shiftL_1_equiv.
+    unfold twoToWsize.
+    rewrite Zdouble_shiftl.
+    f_equal.
+    lia.
+    lia.
+    lia.
+    lia.
 
-  Admitted.
+    rewrite bvMul_2_shiftl_equiv.
+    rewrite shiftL_shiftL.
+    rewrite bvToInt_shiftL_1_equiv.
+    rewrite Z.shiftl_mul_pow2.
+    apply Z.mul_pos_pos.
+    lia.
+    apply Z.pow_pos_nonneg.
+    lia.
+    lia.
+    lia.
+    lia.
 
-  Theorem mod_drop_equiv : forall s1 m a,
-    (Z.modulo (bvToInt _ a) (Z.shiftl 1 (Z.of_nat m))) =
-    (bvToInt _ (drop Bool s1 m a)).
- 
-    intros.
+    rewrite bvMul_2_shiftl_equiv.
+    rewrite shiftL_shiftL.
+    rewrite bvToInt_shiftL_1_equiv.
+    rewrite Z.shiftl_mul_pow2.
+    rewrite Z.mul_1_l.
+    apply Z.pow_le_mono.
+    lia.
+    lia.
+    lia.
+    lia.
+
+    rewrite sbvToInt_shiftL_1_equiv.
+    reflexivity.
+    lia.
+    lia.
+    lia.
+
+    intuition idtac.  
+    eapply Z.le_trans.
+    apply Z.opp_nonpos_nonneg.
+    apply Z.pow_nonneg.
+    lia.
+    rewrite sbvToInt_bvURem_equiv.
+    apply Z.mod_pos_bound.
+    rewrite bvMul_2_shiftl_equiv.
+    rewrite shiftL_shiftL.
+    rewrite bvToInt_shiftL_1_equiv.
+    rewrite Z.shiftl_mul_pow2.
+    rewrite Z.mul_1_l.
+    apply Z.pow_pos_nonneg.
+    lia.
+    lia.
+    lia.
+    lia.
+    lia.
+    rewrite bvMul_2_shiftl_equiv.
+    rewrite shiftL_shiftL.
+    rewrite bvToInt_shiftL_1_equiv.
+    rewrite Z.shiftl_mul_pow2.
+    rewrite Z.mul_1_l.
+    apply Z.pow_pos_nonneg.
+    lia.
+    lia.
+    lia.
+    lia.
+
+    rewrite bvMul_2_shiftl_equiv.
+    rewrite shiftL_shiftL.
+    rewrite bvToInt_shiftL_1_equiv.
+    rewrite Z.shiftl_mul_pow2.
+    rewrite Z.mul_1_l.
+    apply Z.pow_le_mono; lia.
+    lia.
+    lia.
+
+    rewrite sbvToInt_bvURem_equiv.
+    eapply Z.lt_le_trans.
+    apply Z.mod_pos_bound.
+    rewrite bvMul_2_shiftl_equiv.
+    rewrite shiftL_shiftL.
+    rewrite bvToInt_shiftL_1_equiv.
+    rewrite Z.shiftl_mul_pow2.
+    rewrite Z.mul_1_l.
+    apply Z.pow_pos_nonneg.
+    lia.
+    lia.
+    lia.
+    lia.
+
+    rewrite bvMul_2_shiftl_equiv.
+    rewrite shiftL_shiftL.
+    rewrite bvToInt_shiftL_1_equiv.
+    rewrite Z.shiftl_mul_pow2.
+    rewrite Z.mul_1_l.
+    apply Z.pow_le_mono.
+    lia.
+    lia.
+    lia.
+    lia.
+    lia.
+
+    rewrite bvMul_2_shiftl_equiv.
+    rewrite shiftL_shiftL.
+    rewrite bvToInt_shiftL_1_equiv.
+    rewrite Z.shiftl_mul_pow2.
+    rewrite Z.mul_1_l.
+    apply Z.pow_pos_nonneg.
+    lia.
+    lia.
+    lia.
+    lia.
+
+    rewrite bvMul_2_shiftl_equiv.
+    rewrite shiftL_shiftL.
+    rewrite bvToInt_shiftL_1_equiv.
+    rewrite Z.shiftl_mul_pow2.
+    rewrite Z.mul_1_l.
+    apply Z.pow_le_mono.
+    lia.
+    lia.
+    lia.
+    lia.
+
+    intuition idtac.
+    eapply Z.le_trans.
+    apply Z.opp_nonpos_nonneg.
+    apply Z.pow_nonneg.
+    lia.
+    rewrite sbvToInt_shiftL_1_equiv.
+    rewrite Z.shiftl_mul_pow2.
+    rewrite Z.mul_1_l.
+    apply Z.pow_nonneg.
+    lia.
+    lia.
+    lia.
+    lia.
+    rewrite sbvToInt_shiftL_1_equiv.
+    rewrite Z.shiftl_mul_pow2.
+    rewrite Z.mul_1_l.
+    apply Z.pow_lt_mono_r.
+    lia.
+    lia.
+    lia.
+    lia.
+    lia.
+    lia.
+
+    rewrite sbvToInt_bvSub_equiv.
+    rewrite sbvToInt_bvURem_equiv.
+    rewrite bvMul_2_shiftl_equiv.
+    rewrite shiftL_shiftL.
+    rewrite bvToInt_shiftL_1_equiv.
+    rewrite Z.shiftl_mul_pow2.
+    rewrite sbvToInt_shiftL_1_equiv.
+    rewrite Z.mul_1_l.
+    apply Z_sub_range_le_lt_pos.
+    lia.
+    intuition idtac.
+    apply Z.mod_pos_bound.
+    apply Z.pow_pos_nonneg; lia.
+    eapply Z.lt_le_trans.
+    apply Z.mod_pos_bound.
+    apply Z.pow_pos_nonneg; lia.
+    apply Z.pow_le_mono_r.
+    lia.
+    lia.
+    rewrite Z.shiftl_1_l.
+    intuition idtac.
+    apply Z.pow_nonneg; lia.
+    apply Z.pow_lt_mono_r.
+    lia.
+    lia.
+    lia.
+    lia.
+    lia.
+    lia.
+    lia.
+    lia.
+
+    rewrite bvMul_2_shiftl_equiv.
+    rewrite shiftL_shiftL.
+    rewrite bvToInt_shiftL_1_equiv.
+    rewrite Z.shiftl_mul_pow2.  
+    rewrite Z.mul_1_l.
+    apply Z.pow_pos_nonneg; lia.
+    lia.
+    lia.
     
+    rewrite bvMul_2_shiftl_equiv.
+    rewrite shiftL_shiftL.
+    rewrite bvToInt_shiftL_1_equiv.
+    rewrite Z.shiftl_mul_pow2.  
+    rewrite Z.mul_1_l.
+    apply Z.pow_le_mono_r; lia.
+    lia.
+    lia.
+    lia.
 
-  Admitted.
+    rewrite sbvToInt_bvURem_equiv.
+    rewrite bvMul_2_shiftl_equiv.
+    rewrite shiftL_shiftL.
+    rewrite bvToInt_shiftL_1_equiv.
+    rewrite Z.shiftl_mul_pow2.
+    rewrite Z.mul_1_l.
+    intuition idtac.
+    eapply Z.le_trans.
+    apply Z.opp_nonpos_nonneg.
+    apply Z.pow_nonneg; lia.
+    apply Z.mod_pos_bound.
+    apply Z.pow_pos_nonneg; lia.
+    eapply Z.lt_le_trans.
+    apply Z.mod_pos_bound.
+    apply Z.pow_pos_nonneg; lia.
+    apply Z.pow_le_mono_r; lia.
+    lia.
+    lia.
+    lia.
+    rewrite bvMul_2_shiftl_equiv.
+    rewrite shiftL_shiftL.
+    rewrite bvToInt_shiftL_1_equiv.
+    rewrite Z.shiftl_mul_pow2.
+    rewrite Z.mul_1_l.
+    apply Z.pow_pos_nonneg; lia.
+    lia.
+    lia.
 
+    rewrite bvMul_2_shiftl_equiv.
+    rewrite shiftL_shiftL.
+    rewrite bvToInt_shiftL_1_equiv.
+    rewrite Z.shiftl_mul_pow2.
+    rewrite Z.mul_1_l.
+    apply Z.pow_le_mono_r; lia.
+    lia.
+    lia.
 
-  Theorem bvToInt_sbvToInt_equiv : forall n v,
-    n > 0 ->
-    (bvToInt n v < Z.pow 2 (Z.of_nat (pred n)))%Z ->
-    (sbvToInt n v = bvToInt n v).
+    rewrite sbvToInt_shiftL_1_equiv.
+    rewrite Z.shiftl_mul_pow2.
+    rewrite Z.mul_1_l.
+    intuition idtac.
+    eapply Z.le_trans.
+    apply Z.opp_nonpos_nonneg.
+    apply Z.pow_nonneg; lia.
+    apply Z.pow_nonneg; lia.
+    apply Z.pow_lt_mono_r.
+    lia.
+    lia.
+    lia.
+    lia.
+    lia.
 
-    intros.
-    unfold sbvToInt, bvToInt, spec.toZ, spec.toPosZ.
-    destruct n. lia.
-    case_eq (spec.splitmsb (bvToBITS v)); intros.
-    destruct b0.
+    lia.
+    
+    rewrite bvMul_2_shiftl_equiv.
+    rewrite shiftL_shiftL.
+    match goal with
+    | [|- _ = spec.toZ (bvToBITS ?a)] =>
+    replace (spec.toZ (bvToBITS a)) with (sbvToInt _ a)
+    end.
+    rewrite sbvToInt_shiftR_equiv.
+    repeat rewrite sbvToInt_bvSub_equiv.
+    rewrite sbvToInt_bvURem_equiv.
+    rewrite bvToInt_shiftL_1_equiv.
+    rewrite Z.shiftl_mul_pow2.
+    rewrite Z.mul_1_l.
+    rewrite Z.shiftr_div_pow2.
+    
+    f_equal.
+    f_equal.
+    congruence.
+    f_equal.
+    unfold twoToWsize.
+    rewrite Zdouble_shiftl.
+    rewrite Z.shiftl_1_l.
+    f_equal.
+    f_equal.
+    lia.
+    lia.
+    rewrite sbvToInt_shiftL_1_equiv.
+    reflexivity.
+    lia.
+    lia.
+    unfold twoToWsize.
+    rewrite Z.shiftl_1_l.
+    reflexivity.
 
-  Admitted.
+    lia.
+    lia.
+    lia.
+    lia.
+    
+    (* a nuch of size checks *)
+    admit.
+    admit.
+    lia.
+    admit.
+    admit.
+    lia.
+    admit.
+    admit.
+    lia.
+    admit.
+    admit.
+    lia.
+    admit.
 
-  Theorem shiftR_bvToInt_nonneg : 
-    forall n s x,
-    s > 0 ->
-    (VectorDef.hd (shiftR (S n) bool false x s) = false).
+  Abort.
+*)
 
-  Admitted.
 
   Theorem fiat_mul_scalar_rwnaf_odd_loop_body_gen_snd_nonneg : 
     forall wsize x, 
@@ -816,174 +1649,6 @@ Section ECEqProof.
       let n' := (shiftR _ _ false (bvSub _ n k_i) wsize) in
       (drop _ 368 16 k_i) :: (recode_rwnaf_odd_bv wsize nw' n')
     end.
-
-
-  Theorem bvToInt_drop_equiv : forall n1 n2 x,
-    ((bvToInt _ x) < Z.pow 2 (Z.of_nat n2))%Z ->
-    bvToInt _ (drop _ n1 n2 x) = bvToInt _ x.
-
-  Admitted.
-
-  Theorem sbvToInt_drop_equiv : forall n1 n2 x,
-    n2 > 0 -> 
-    (-(Z.pow 2 (Z.of_nat (pred n2))) <= (sbvToInt _ x) < Z.pow 2 (Z.of_nat (pred n2)))%Z ->
-    sbvToInt _ (drop _ n1 n2 x) = sbvToInt _ x.
-
-  Admitted.
-
-  Theorem sbvToInt_bvSub_equiv : forall n v1 v2,
-    n > 1 -> 
-      (-(Z.pow 2 (Z.of_nat (pred (pred n)))) <= (sbvToInt _ v1) < Z.pow 2 (Z.of_nat (pred (pred n))))%Z ->
-     (-(Z.pow 2 (Z.of_nat (pred (pred n)))) <= (sbvToInt _ v2) < Z.pow 2 (Z.of_nat (pred (pred n))))%Z ->
-    sbvToInt _ (bvSub n v1 v2) = ((sbvToInt _ v1) - (sbvToInt _ v2))%Z.
-
-  Admitted.
-
-  Theorem bvToInt_intToBv_id : forall n v,
-    bvToInt n (intToBv n v) = v.
-
-  Admitted.
-
-  Theorem sbvToInt_intToBv_id : forall n v,
-    (-Z.pow 2 (Z.of_nat (pred n)) <= v < Z.pow 2 (Z.of_nat (pred n)))%Z ->
-    sbvToInt n (intToBv n v) = v.
-
-  Admitted.
-
-  Theorem sbvToInt_bvURem_equiv : forall n v1 v2,
-    n > 0 ->
-    (0 < bvToInt _ v2)%Z ->
-    (bvToInt _ v2 <= Z.pow 2 (Z.of_nat (pred n)))%Z ->
-    sbvToInt n (bvURem _ v1 v2) = Z.modulo (bvToInt _ v1) (bvToInt _ v2).
-
-    intros.
-    Local Transparent bvURem.
-    unfold bvURem.
-    destruct n. lia.
-    rewrite bvToInt_sbvToInt_equiv.
-    apply bvToInt_intToBv_id.
-    trivial.
-    rewrite bvToInt_intToBv_id.
-    eapply Z.lt_le_trans.
-    eapply Z.mod_pos_bound.
-    trivial.
-    trivial.
-  Qed.
-
-  Theorem bvToInt_drop_le : forall n1 n2 v,
-    (bvToInt _ (drop _ n1 n2 v) <= bvToInt _ v)%Z.
-
-  Admitted.
-
-  Theorem bvMul_2_shiftl_equiv : forall n v,
-    bvMul n (intToBv _ 2) v = shiftL _ _ false v 1.
-  Admitted.
-
-  Theorem shiftL_shiftL : forall (A : Type) n (b : A) v n1 n2,
-    (shiftL n _ b (shiftL n _ b v n1) n2) = shiftL n _ b v (n1 + n2).
-  Admitted.
-
-  Theorem bvToInt_shiftL_1_equiv : forall n s,
-    s < n ->
-    bvToInt n (shiftL _ _ false (intToBv _ 1) s) = 
-    Z.shiftl 1 (Z.of_nat s).
-  Admitted.
-
-  Theorem sbvToInt_shiftL_1_equiv : forall n s,
-    n > 0 ->
-    s < pred n ->
-    sbvToInt n (shiftL _ _ false (intToBv _ 1) s) = 
-    Z.shiftl 1 (Z.of_nat s).
-  Admitted.
-
-  Theorem bvToInt_bvSub_nonneg_equiv : forall n v1 v2,
-    (bvToInt _ v2 <= bvToInt _ v1)%Z ->
-    (bvToInt n (bvSub _ v1 v2)) =
-    ((bvToInt _ v1) - (bvToInt _ v2))%Z.
-  Admitted.
-
-  Theorem bvToBITS_bitsToBv_id : forall n v,
-    bvToBITS (@bitsToBv n v) = v.
-  Admitted.
-
-  Theorem toZ_toPosZ_equiv : forall n (v : spec.BITS (S n)),
-    (spec.toZ v mod 2 ^ Z.of_nat (S n) = spec.toPosZ v mod 2 ^ Z.of_nat (S n))%Z.
-  Admitted.
-
-  Theorem toPosZ_addB_equiv: forall n (v1 v2 : spec.BITS (S n)),
-    (0 <= spec.toPosZ v1 + spec.toZ v2 < Z.pow 2 (Z.of_nat (S n)))%Z ->
-    spec.toPosZ (addB v1 v2) =
-    (spec.toPosZ v1 + spec.toZ v2)%Z.
-
-    intros.
-    erewrite <- (@Zdiv.Zmod_small (spec.toPosZ v1 + spec.toZ v2)); eauto.
-    rewrite <- Zdiv.Zplus_mod_idemp_r.
-    rewrite toZ_toPosZ_equiv.
-    rewrite Zdiv.Zplus_mod_idemp_r.
-   
-    rewrite addB_def.
-  Admitted.
-
-
-  Theorem sbvToInt_bvNeg_equiv : forall n v,
-    sbvToInt n (bvNeg _ v) = Z.opp (sbvToInt _ v).
-  Admitted.
-
-  Theorem bvToInt_bvAdd_small_equiv : forall n (v1 v2 : bitvector n),
-    (* (sbvToInt _ v2 <= bvToInt _ v1)%Z -> *)
-    (0 <= (bvToInt _ v1) + (sbvToInt _ v2) < Z.pow 2 (Z.of_nat n))%Z->
-    (bvToInt n (bvAdd _ v1 v2)) =
-    ((bvToInt _ v1) + (sbvToInt _ v2))%Z.
-
-    intros.
-    unfold bvToInt, sbvToInt in *.
-    destruct n.
-    (* empty bit vectors *)
-    admit.
-
-    Local Transparent bvAdd operations.adcB.
-    unfold bvAdd.
-    rewrite bvToBITS_bitsToBv_id.
-    apply toPosZ_addB_equiv.
-    apply H.
-
-  Admitted.
-
-  
-
-  Theorem bvToInt_bvSub_small_equiv : forall n v1 v2,
-    (0 <= (bvToInt _ v1) - (sbvToInt _ v2) < Z.pow 2 (Z.of_nat n))%Z->
-    (bvToInt n (bvSub _ v1 v2)) =
-    ((bvToInt _ v1) - (sbvToInt _ v2))%Z.
-
-    intros.
-    rewrite bvSub_eq_bvAdd_neg.
-    rewrite <- Z.add_opp_r.
-    rewrite bvToInt_bvAdd_small_equiv.
-    rewrite sbvToInt_bvNeg_equiv.
-    reflexivity.
-    
-    rewrite sbvToInt_bvNeg_equiv.
-    rewrite Z.add_opp_r.
-    trivial.
-  Qed.
-
-(*
-  Theorem bvToInt_shiftL_1_pos : forall n s,
-    s < n ->
-    (0 < bvToInt n (shiftL _ _ false (intToBv _ 1) s))%Z.
-  Admitted.
-
-  Theorem bvToInt_shiftL_1_small : forall n s,
-    s < n ->
-    (bvToInt n (shiftL _ _ false (intToBv _ 1) s) <= Z.pow 2 (Z.of_nat s))%Z.
-  Admitted.
-*)
-  Theorem bvToInt_shiftR_lt : forall n v s b,
-    ((bvToInt n v) < (Z.pow 2 (Z.of_nat s + b)))%Z ->
-    ((bvToInt n (shiftR _ _ false v s)) < Z.pow 2 b)%Z.
-
-  Admitted.
 
   Local Opaque sbvToInt.
 
@@ -1058,38 +1723,70 @@ Section ECEqProof.
     lia.
 
   Qed.
+
   
-  Theorem bvToInt_nonneg : forall n v,
-    (0 <= bvToInt n v)%Z.
+  Theorem Z_sub_range_le_lt_dbl_pos : forall x y,
+    (0 <= x ->
+    0 <= y < 2 * x ->
+    -x <= y - x < x)%Z.
+
+    intros.
+    lia.
+  
+  Qed.
+
+  Theorem bound_gen : forall x1 x2 y1 y2 z,
+    (x1 <= z < y1 ->
+    x2 <= x1 ->
+    y1 <= y2 ->
+    x2 <= z < y2)%Z.
+
+    intuition idtac.
+    eapply Z.le_trans; eauto.
+    eapply Z.lt_le_trans; eauto.
+
+  Qed.
+
+  Theorem bvToInt_sbvToInt_range : forall n v x,
+    (bvToInt n v < 2^(1 + x) ->
+    -2^x <= sbvToInt _ v < 2^x)%Z.
+  Admitted.
+
+  Theorem bvToInt_shiftR_equiv
+     : forall (n s : nat) (x : t bool n),
+       s >= 0 ->
+       bvToInt n (shiftR n bool false x s) =
+       BinInt.Z.shiftr (bvToInt n x)
+         (BinInt.Z.of_nat s).
+
   Admitted.
 
   Theorem recode_rwnaf_odd_bv_equiv : 
     forall wsize nw n,
     0 < wsize < 16 -> 
+    (* bvToInt 384 n = sbvToInt 384 n -> *)
     (bvToInt _ n < (Z.pow 2 (Z.of_nat ((S nw) * wsize))))%Z -> 
     List.Forall2 (fun (x : Z) (y : bitvector 16) => x = (sbvToInt _ y)) 
     (recode_rwnaf_odd wsize nw (bvToInt _ n)) 
     (recode_rwnaf_odd_bv wsize nw n).
 
-
     induction nw; intros.
     econstructor.
+    rewrite sbvToInt_drop_equiv.
     rewrite bvToInt_sbvToInt_equiv.
-    rewrite bvToInt_drop_equiv.
     reflexivity.
-    eapply Z.lt_le_trans.
-    eauto.
+    rewrite SAWCorePreludeExtra.addNat_add.
+    lia.
+    eapply Z.lt_le_trans; eauto.
+    apply Z.pow_le_mono.
+    lia.
+    rewrite SAWCorePreludeExtra.addNat_add.
+    lia.
+    lia.
+    apply bvToInt_sbvToInt_range.
+    eapply Z.lt_le_trans; eauto.
     apply Z.pow_le_mono_r.
     lia.
-    lia.
-    lia.
-    eapply Z.le_lt_trans.
-    apply bvToInt_drop_le.
-    eapply Z.lt_le_trans.
-    apply H0.
-    apply Z.pow_le_mono_r.
-    lia.
-    simpl.
     lia.
     econstructor.
 
@@ -1103,7 +1800,73 @@ Section ECEqProof.
              (shiftL 384 bool false (intToBv 384%nat 1) (wsize + 1)))
           (shiftL 384 bool false (intToBv 384%nat 1) wsize)) <
      2 ^ Z.of_nat wsize)%Z).
-    admit.
+    rewrite sbvToInt_bvSub_equiv.
+    rewrite sbvToInt_bvURem_equiv.
+    rewrite sbvToInt_shiftL_1_equiv.
+    rewrite Z.shiftl_1_l.
+    apply Z_sub_range_le_lt_dbl_pos.
+    apply Z.pow_nonneg; lia.
+    rewrite bvToInt_shiftL_1_equiv.
+    rewrite Z.shiftl_1_l.
+    rewrite Znat.Nat2Z.inj_add.
+    rewrite Z.pow_add_r.
+    rewrite Z.mul_comm.
+    apply Z.mod_pos_bound.
+    apply Z.mul_pos_pos; try lia.
+    apply Z.pow_pos_nonneg; lia.
+    lia.
+    lia.
+    lia.
+    lia.
+    lia.
+    lia.
+    rewrite bvToInt_shiftL_1_equiv.
+    rewrite Z.shiftl_1_l.
+    apply Z.pow_pos_nonneg; lia.
+    lia.
+    rewrite bvToInt_shiftL_1_equiv.
+    rewrite Z.shiftl_1_l.
+    apply Z.pow_le_mono; lia.
+    lia.
+    lia.
+    rewrite sbvToInt_bvURem_equiv.
+    rewrite bvToInt_shiftL_1_equiv.
+    rewrite Z.shiftl_1_l.
+    rewrite Znat.Nat2Z.inj_add.
+    rewrite Z.pow_add_r.
+    rewrite Z.mul_comm.
+    eapply bound_gen.
+    apply Z.mod_pos_bound.
+    apply Z.mul_pos_pos; try lia;
+    apply Z.pow_pos_nonneg; lia.
+    apply Z.opp_nonpos_nonneg.
+    apply Z.pow_nonneg; lia.
+    rewrite <- Z.pow_add_r.
+    apply Z.pow_le_mono; lia.
+    lia.
+    lia.
+    lia.
+    lia.
+    lia.
+    lia.
+    rewrite bvToInt_shiftL_1_equiv.
+    rewrite Z.shiftl_1_l.
+    apply Z.pow_pos_nonneg; lia.
+    lia.
+    rewrite bvToInt_shiftL_1_equiv.
+    rewrite Z.shiftl_1_l.
+    apply Z.pow_le_mono; lia.
+    lia.
+    rewrite sbvToInt_shiftL_1_equiv.
+    rewrite Z.shiftl_1_l.
+    intuition idtac.
+    eapply Z.le_trans.
+    apply Z.opp_nonpos_nonneg.
+    apply Z.pow_nonneg; lia.
+    apply Z.pow_nonneg; lia.
+    apply Z.pow_lt_mono_r; lia.
+    lia.
+    lia.
 
     match goal with
     | [|- List.Forall2 _ (?a :: _) (?b :: _)] =>
@@ -1119,9 +1882,7 @@ Section ECEqProof.
     f_equal.
     rewrite sbvToInt_bvURem_equiv; try lia.
     rewrite bvToInt_shiftL_1_equiv; try lia.
-    f_equal.
-    rewrite Znat.Nat2Z.inj_add.
-    reflexivity.
+    f_equal. f_equal. lia.
     rewrite bvToInt_shiftL_1_equiv; try lia.
     rewrite Z.shiftl_1_l.
     apply Z.pow_pos_nonneg; lia.
@@ -1174,7 +1935,6 @@ Section ECEqProof.
     apply Z.pow_nonneg; lia.
     apply Z.pow_nonneg; lia.
     apply Z.pow_lt_mono_r; simpl; lia.
-    simpl; lia.
 
     split.
     eapply Z.le_trans; [idtac | apply H1].
@@ -1195,11 +1955,54 @@ Section ECEqProof.
     assert (a = (bvToInt _ b))
     end.
 
-    admit.
+    rewrite bvMul_2_shiftl_equiv.
+    rewrite shiftL_shiftL.
+    rewrite bvToInt_shiftR_equiv.
+    rewrite bvToInt_bvSub_small_equiv.
+    rewrite sbvToInt_bvSub_equiv.
+    rewrite sbvToInt_bvURem_equiv.
+    rewrite bvToInt_shiftL_1_equiv.
+    rewrite Z.shiftl_mul_pow2.
+    rewrite Z.mul_1_l.
+    rewrite Z.shiftr_div_pow2.
+ 
+    f_equal.
+    f_equal.
+    f_equal.
+    unfold twoToWsize.
+    rewrite Zdouble_shiftl.
+    rewrite Z.shiftl_1_l.
+    f_equal.
+    f_equal.
+    lia.
+    lia.
+    rewrite sbvToInt_shiftL_1_equiv.
+    reflexivity.
+    lia.
+    lia.
+    unfold twoToWsize.
+    rewrite Z.shiftl_1_l.
+    reflexivity.
 
+    lia.
+    lia.
+    lia.
+    lia.
+    
+    (* a bunch of size checks *)
+    admit.
+    admit.
+    lia.
+    admit.
+    admit.
+    (* This is the complicated one that we proved somewhere else*)
+    admit.
+    lia.
+   
     rewrite H3.
     eapply IHnw.
     lia.
+    
     apply bvToInt_shiftR_lt.
 
     rewrite bvToInt_bvSub_small_equiv.
@@ -1219,10 +2022,9 @@ Section ECEqProof.
     eauto.
     simpl.
     lia.
-    simpl. lia.
   (* 2 * 2 ^wsize is positive *)
     admit.
-    (* 2 * 2^wsize < 2^384 *)
+    (* 2 * 2^wsize <= 2^383 *)
     admit.
 
     rewrite sbvToInt_bvURem_equiv; try lia.
@@ -1299,11 +2101,9 @@ Section ECEqProof.
     (* integers from 384 bit vectors are less than 2^384 *)
     admit.
 
-    simpl.
-    lia.
   (* 2 * 2 ^wsize is positive *)
     admit.
-    (* 2 * 2^wsize < 2^384 *)
+    (* 2 * 2^wsize <= 2^383 *)
     admit.
 
     rewrite sbvToInt_bvURem_equiv; try lia.
@@ -1355,7 +2155,7 @@ Section ECEqProof.
   Admitted.
 
 
- Definition recode_rwnaf_odd_bv_scanl_fix_body wsize n :=
+  Definition recode_rwnaf_odd_bv_scanl_fix_body wsize n :=
       let k_i := (bvSub _ (bvURem _ n (bvMul _ (bvNat _ 2) (shiftL _ _ false (bvNat _ 1%nat) wsize))) (shiftL _ _ false (bvNat _ 1%nat) wsize)) in
       let n' := (shiftR _ _ false (bvSub _ n k_i) wsize) in
       ((drop _ 368 16 k_i), n').
@@ -1384,56 +2184,6 @@ Section ECEqProof.
 
   Qed.
 
-  Theorem forall2_symm : forall (A B : Type)(P : B -> A -> Prop) lsa lsb,
-    List.Forall2 (fun a b => P b a) lsa lsb ->
-    List.Forall2 P lsb lsa.
-  
-    induction 1; intros;
-    econstructor; eauto.
-
-  Qed.
-
-  Theorem forall2_trans : forall ( A B C : Type)(R1 : A -> B -> Prop)(R2 : B -> C -> Prop)(R3 : A -> C -> Prop)
-    lsa lsb lsc,
-    List.Forall2 R1 lsa lsb ->
-    (forall a b c, R1 a b -> R2 b c -> R3 a c) ->
-    List.Forall2 R2 lsb lsc ->
-    List.Forall2 R3 lsa lsc.
-
-    induction lsa; intuition; simpl in *.
-    inversion H; subst.
-    inversion H1; subst.
-    econstructor.
-
-    inversion H; subst.
-    inversion H1; subst.
-    econstructor.
-    eauto.
-    eapply IHlsa; eauto.
-
-  Qed.
-
-  Theorem forall2_eq : forall (A : Type)(ls1 ls2 : list A),
-    ls1 = ls2 ->
-    List.Forall2 eq ls1 ls2.
-
-    induction ls1; intros; simpl in *; subst.
-    econstructor.
-
-    econstructor; trivial.
-    eauto.
-
-  Qed.
-
-  Theorem forall2_map_eq : forall (A B : Type)(f : B -> A) lsa lsb,
-    List.Forall2 (fun a b => a = f b) lsa lsb ->
-    lsa = List.map f lsb.
-
-    induction 1; intros; simpl in *; trivial.
-    congruence.
-
-  Qed.
-
   Theorem recode_rwnaf_odd_bv_scanl_fix_body_fiat_equiv : forall wsize z, 
     recode_rwnaf_odd_bv_scanl_fix_body wsize z = 
     fiat_mul_scalar_rwnaf_odd_loop_body_gen wsize z.
@@ -1447,6 +2197,7 @@ Section ECEqProof.
 
   Theorem fiat_mul_scalar_rwnaf_odd_gen_equiv : forall nw wsize z,
     0 < wsize < 16 ->
+    (* bvToInt _ z = sbvToInt _ z -> *)
     (bvToInt 384%nat z < 2 ^ Z.of_nat (S (S (S nw)) * wsize))%Z ->
     List.Forall2 (fun (x : Z) (y : bitvector 16) => x = (sbvToInt _ y))
   (recode_rwnaf_odd wsize (S (S nw)) (bvToInt _ z))
@@ -1459,6 +2210,7 @@ Section ECEqProof.
     lia.
     intros; subst.
     trivial.
+    intros; subst; trivial.
     apply forall2_eq.
 
     unfold fiat_mul_scalar_rwnaf_odd_gen.
@@ -1482,14 +2234,10 @@ Section ECEqProof.
     
   Qed.
 
-  Theorem bvOr_bvToInt_equiv : forall n x y,
-    bvToInt n (bvOr n x y) =
-    BinInt.Z.lor (bvToInt n x) (bvToInt n y).
-  Admitted.
-
   Theorem fiat_mul_scalar_rwnaf_gen_equiv : forall nw wsize z,
     0 < wsize < 16 ->
     (bvToInt 384%nat z < 2 ^ Z.of_nat (S (S (S nw)) * wsize))%Z ->
+   (*  sbvToInt _ z = bvToInt _ z -> *)
     List.Forall2 (fun x (y : bitvector 16) => x = (sbvToInt _ y))
     (recode_rwnaf wsize (S (S (S nw))) (bvToInt _ z)) 
     (fiat_mul_scalar_rwnaf_gen wsize nw z).
@@ -1500,6 +2248,7 @@ Section ECEqProof.
       (bvToInt _ (bvOr 384 z (intToBv 384 1))).
     apply fiat_mul_scalar_rwnaf_odd_gen_equiv.
     lia.
+  
     rewrite bvOr_bvToInt_equiv.
     rewrite bvToInt_intToBv_id.
     case_eq (BinInt.Z.odd (bvToInt 384%nat z)); intros.
@@ -1533,25 +2282,6 @@ Section ECEqProof.
 
   Qed.
 
-(*
-  Definition numWindows := 55.
-  Definition wsize := 7.
-
-  Theorem wsize_nz : wsize <> 0%nat.
-    unfold wsize in *.
-    intuition.
-    discriminate.
-  Qed.
-
-  Theorem numWindows_nz : numWindows <> 0%nat.
-
-    unfold numWindows in *.
-    intuition.
-    discriminate.
-
-  Qed.
-*)
-
   Theorem Proper_opp : Proper (Jacobian.eq ==> Jacobian.eq) (@Jacobian.opp F Feq Fzero Fone Fopp Fadd Fsub Fmul Finv Fdiv a b F_Field Feq_dec).
   Admitted.
 
@@ -1565,43 +2295,6 @@ Section ECEqProof.
     jac_eq (seqToProd (EC_fiat_P384_7.conditional_subtract_if_even_ct Fsquare Fmul Fsub Fadd
         Fopp p1 n p2)) (seqToProd (if (Nat.even (bvToNat _ n)) then (fiat_point_add false p1 (fiat_point_opp p2)) else p1)).
   Admitted.
-
-(*
-  Theorem groupMul_signedWindows_equiv: forall n t1 t2,
-    List.Forall2 (fun x y => jac_eq (fromPoint x) (seqToProd y)) t1 (seqToList t2) ->
-    jac_eq
-  (fromPoint
-     (groupMul_signedWindows Jacobian.add zero_point
-        Jacobian.double wsize
-        (groupMul_signed_table zero_point Jacobian.opp
-           t1)
-        (recode_rwnaf wsize numWindows (bvToInt _ n))))
-  (seqToProd
-     (ecFoldl 54 (seq 3 (seq 6 (seq 64 Bool))) 
-        (seq 16 Bool)
-        (fiat_double_add_body Fsquare Fmul Fsub Fadd Fopp t2)
-        (fiat_select_point_ct
-           (sign_extend_16_64
-              (ecSShiftR 16 Integer PIntegralInteger
-                 (ecAt 55 (seq 16 Bool) Integer
-                    PIntegralInteger
-                    (fiat_mul_scalar_rwnaf n)
-                    (ecDiv Integer PIntegralInteger
-                       (ecNumber 384 Integer PLiteralInteger)
-                       (ecNumber 7 Integer PLiteralInteger)))
-                 (ecNumber 1%nat Integer PLiteralInteger)))
-           t2)
-        (ecDrop 1%nat 54 (seq 16 Bool)
-           (coerce (seq 55 (seq 16 Bool))
-              (seq (tcAdd 1%nat 54) (seq 16 Bool))
-              (seq_cong1 55 (tcAdd 1%nat 54) 
-                 (seq 16 Bool)
-                 (reflexivity (tcAdd 1%nat 54)))
-              (ecReverse 55 (seq 16 Bool)
-                 (fiat_mul_scalar_rwnaf n)))))).
-
-  Admitted.
-  *)
 
   Theorem fiat_pre_comp_table_0 : forall p,
     (ecAt 64 (seq 3 (seq 6 (seq 64 Bool))) Integer
@@ -1625,34 +2318,6 @@ Section ECEqProof.
     destruct p. 
     apply jac_eq_refl.
   Qed.
-
-  Theorem fold_left_unroll_one : forall (A B : Type) def (f : A -> B -> A) (ls : list B) a,
-    (List.length ls > 0)%nat ->
-    List.fold_left f ls a = List.fold_left f (List.tl ls) (f a (List.hd def ls)).
-
-    destruct ls; intros; simpl in *.
-    lia.
-    reflexivity.
-
-  Qed.
-
-  Theorem fold_left_R : forall (A1 A2 B1 B2 : Type)(RA : A1 -> A2 -> Prop)(RB : B1 -> B2 -> Prop)(f1 : A1 -> B1 -> A1)(f2: A2 -> B2 -> A2) ls1 ls2 a1 a2,
-    RA a1 a2 ->
-    List.Forall2 RB ls1 ls2 ->
-    (forall a1 a2 b1 b2, RA a1 a2 -> RB b1 b2 -> RA (f1 a1 b1) (f2 a2 b2)) ->
-    RA (List.fold_left f1 ls1 a1) (List.fold_left f2 ls2 a2).
-
-    induction ls1; destruct ls2; intros; simpl in *; trivial.
-    inversion H0.
-    inversion H0.
-    inversion H0; subst; clear H0.
-    eapply IHls1.
-    eapply H1; eauto.
-    trivial.
-    eauto.
-
-  Qed.
-
 
   Theorem fiat_selext_point_ct_gen_nth_equiv_h : forall ls n a,
     List.fold_left
@@ -1679,23 +2344,9 @@ Section ECEqProof.
     (* apply fiat_selext_point_ct_gen_nth_equiv_h. *)
   Admitted.
 
-  Theorem bvSShr_intToBv_equiv : forall n z v,
-    bvSShr _ (intToBv (S n) z) v = intToBv (S n) (Z.shiftr z (Z.of_nat v)).
-  Admitted.
-
   Theorem sign_extend_16_64_intToBv_equiv : forall z,
     sign_extend_16_64 (intToBv 16 z) = intToBv 64 z.
   Admitted.
-
-  Theorem hd_rev_eq_last : forall (A : Type)(ls : list A)(def : A),
-    List.hd def (List.rev ls) = List.last ls def.
-  
-    induction ls using rev_ind; intros; simpl in *; trivial.
-    rewrite rev_unit.
-    simpl.
-    rewrite last_last.
-    reflexivity.
-  Qed.
 
   Theorem groupDouble_n_zero : forall n,
     groupDouble_n Jacobian.double n zero_point == zero_point.
@@ -1710,132 +2361,7 @@ Section ECEqProof.
     reflexivity.
   Qed.
 
-  Theorem recode_rwnaf_odd_length : forall w nw z,
-    List.length (recode_rwnaf_odd w nw z) = (S nw).
-
-    induction nw; intros; simpl in *; trivial.
-    rewrite IHnw.
-    trivial.
-
-  Qed.
-
-  Theorem recode_rwnaf_length : forall w nw z,
-    nw <> 0%nat -> 
-    List.length (recode_rwnaf w nw z) = nw.
-
-    intros.
-    destruct nw.
-    lia.
-    apply recode_rwnaf_odd_length.
-
-  Qed.
-
-  Theorem fold_left_scanl_app_equiv : forall (A B : Type) (f : A -> B -> A) ls def a1 a2,
-    a2 <> List.nil ->
-    List.fold_left
-  (fun (x : list A) (y : B) =>
-   x ++ [f (List.last x def) y]) ls 
-  (List.cons a1 a2) =
-    a1 :: (List.fold_left (fun (x : list A) (y : B) =>
-   x ++ [f (List.last x def) y]) ls 
-  a2 ).
-
-    induction ls; intros; simpl in *; trivial.
-    rewrite (@IHls _ a1).
-    destruct a2.
-    intuition idtac.
-    reflexivity.
-    f_equal.
-    intuition idtac.
-    apply app_eq_nil in H0.
-    intuition idtac.
-
-  Qed.
-
-  Theorem fold_left_scanl_equiv : forall (A B : Type) def (f : A -> B -> A) ls a,
-    List.fold_left (fun x y => x ++ (f (List.last x def) y)::List.nil) ls [a] = 
-    CryptoToCoq_equiv.scanl f ls a.
-
-    induction ls; intros; simpl in *; trivial.
-    rewrite <- IHls.
-    rewrite fold_left_scanl_app_equiv.
-    reflexivity.
-    congruence.
-  Qed.
-
   Definition fiat_pre_comp_table_gen := fiat_pre_comp_table_gen Fsquare Fmul Fsub Fadd.
-
-  Theorem Forall2_scanl : forall (A1 A2 B1 B2 : Type)(PA : A1 -> A2 -> Prop)(PB : B1 -> B2 -> Prop)
-    (f1 : A1 -> B1 -> A1)(f2 : A2 -> B2 -> A2) ls1 ls2 a1 a2,
-    List.Forall2 PB ls1 ls2 ->
-    (forall a1 a2 b1 b2, PA a1 a2 -> PB b1 b2 -> PA (f1 a1 b1) (f2 a2 b2)) ->
-    PA a1 a2 ->
-    List.Forall2 PA (CryptoToCoq_equiv.scanl f1 ls1 a1) (CryptoToCoq_equiv.scanl f2 ls2 a2).
-
-    induction ls1; destruct ls2; simpl in *; intros.
-    econstructor; eauto.
-    inversion H.
-    inversion H.
-    inversion H; clear H; subst.
-    econstructor; eauto.
-
-  Qed.
-
-  (* Not sure if this is true, but we could always add more assumptions that triples are Jacobian*)
-  Theorem jac_eq_point_ex : forall p1 p2,
-    jac_eq (fromPoint p1) p2 ->
-    exists p2', p2 = fromPoint p2'.
-
-    intros.
-    unfold jac_eq in *.
-    remember (fromPoint p1) as z. destruct z. destruct p.
-    destruct p2. destruct p.
-
-    assert ((fun '(X, Y, Z) =>  if dec (Feq Z Fzero)
-                          then True
-                          else
-                           Feq (Fmul Y Y)
-                             (Fadd
-                                (Fadd (Fmul (Fmul X X) X)
-                                   (Fmul (Fmul a X)
-                                      (Fmul (Fmul Z Z) (Fmul Z Z))))
-                                (Fmul b
-                                   (Fmul (Fmul (Fmul Z Z) Z)
-                                      (Fmul (Fmul Z Z) Z))))) (f3, f4, f2)).
-    destruct (dec (Feq f 0)).
-    rewrite H.
-    destruct (dec (Feq 0 0)).
-    trivial.
-    exfalso.
-    apply n.
-    reflexivity.
-    intuition idtac.
-    destruct (dec (Feq f2 0)).
-    trivial.
-    admit.
- 
-    exists (exist _ _ H0).
-    reflexivity.
-  Admitted.
-
-  Theorem jac_eq_jacobian_eq: forall p1 p2,
-    jac_eq (fromPoint p1) (fromPoint p2) ->
-    Jacobian.eq p1 p2.
-
-    intros. 
-    unfold jac_eq, Jacobian.eq, fromPoint in *.
-    eauto.
-  Qed.
-
-  Theorem Forall2_I : forall (A B : Type)(ls1 : list A)(ls2 : list B),
-    List.length ls1 = List.length ls2 ->
-    List.Forall2 (fun a b => True) ls1 ls2.
-
-    induction ls1; destruct ls2; intros; simpl in *; try lia.
-    econstructor.
-    econstructor; eauto; econstructor.
-
-  Qed.
 
   Theorem preCompTable_equiv_h : forall ls1 ls2 p1 p2,
     List.length ls1 = List.length ls2 ->
@@ -1886,14 +2412,6 @@ Section ECEqProof.
     trivial.
   Qed.
 
-  Theorem forNats_length : forall n,
-    List.length (forNats n) = n.
-
-    induction n; intros; simpl in *; trivial.
-    congruence.
-
-  Qed.
-
   Theorem preCompTable_equiv : forall w p,
     (tableSize w) > 1 ->
     List.Forall2 (fun a b => jac_eq (fromPoint a) (seqToProd b))
@@ -1910,60 +2428,6 @@ Section ECEqProof.
     lia.
     rewrite seqToProd_inv.
     eapply jac_eq_refl.
-  Qed.
-
-
-
-  Theorem Forall2_nth : forall (A B : Type)(P : A -> B -> Prop) lsa lsb,
-    List.Forall2 P lsa lsb ->
-    forall n defA defB,
-    P defA defB ->
-    P (List.nth n lsa defA) (List.nth n lsb defB).
-
-    induction 1; intros; simpl in *.
-    destruct n; trivial.
-    destruct n; trivial.
-    eapply IHForall2; trivial.
-
-  Qed.
-
-  Theorem bvNat_Z_to_nat_eq_intToBv : forall n (z : Z),
-    (0 <= z)%Z ->
-    bvNat n (Z.to_nat z) = intToBv n z.
-  Admitted.
-
-  Theorem skipn_1_eq_tl : forall (A : Type)(ls : list A),
-    skipn 1 ls = List.tl ls.
-
-    intros.
-    destruct ls; trivial.
-
-  Qed.
-
-  Theorem Forall2_tl : forall (A B : Type)(P : A -> B -> Prop) ls1 ls2,
-    List.Forall2 P ls1 ls2 ->
-    List.Forall2 P (List.tl ls1) (List.tl ls2).
-
-    intros.
-    inversion H; clear H; subst;
-    simpl.
-    econstructor.
-    trivial.
-
-  Qed.
-
-  Theorem Forall2_rev : forall (A B : Type)(P : A -> B -> Prop) ls1 ls2,
-    List.Forall2 P ls1 ls2 ->
-    List.Forall2 P (List.rev ls1) (List.rev ls2).
-  
-    induction 1; intros; simpl in *.
-    econstructor.
-    eapply Forall2_app.
-    eauto.
-    econstructor.
-    trivial.  
-    econstructor.
-
   Qed.
 
   Theorem ct_abs_equiv : forall wsize b1 b2,
@@ -2076,22 +2540,94 @@ Section ECEqProof.
 
   Qed.
        
-  Theorem bvToNat_Z_to_nat_equiv : forall n x z,
-    (0 <= z)%Z ->
-    sbvToInt n x = z ->
-    bvToNat n x = Z.to_nat z.
-
-  Admitted.
-
   Theorem sbvToInt_sign_extend_16_64_equiv : forall x,
     sbvToInt _ (sign_extend_16_64 x) = sbvToInt _ x.
 
   Admitted.
 
-  Theorem bvSShr_Z_shiftr_equiv : forall n x1 x2 y1 y2,
-    Z.of_nat y1 = y2 ->
-    sbvToInt _ x1 = x2 ->
-    sbvToInt _ (bvSShr n x1 y1) = Z.shiftr x2 y2.
+  Theorem sbvToInt_nz_nth : forall n (v : Vec n _) n' (nlt : n' < n),
+    nth_order v nlt = true ->
+    sbvToInt _ v <> 0%Z.
+
+  Admitted.
+
+  Search Vector.t.
+    Search shiftR1.
+
+  Print shiftR1.
+  Locate shiftout.
+
+  (*
+
+  Theorem shiftR1_cons_eq : forall (A : Type)(n : nat)(v : Vec n A) a1 a2,
+    shiftR1 _ _ a2 (Vector.cons _ a1 _ v) = VectorDef.shiftin a2 v.
+
+    induction v; intros.
+    reflexivity.
+  
+    simpl.
+    erewrite <- IHv.
+    unfold shiftR1.
+    simpl.
+    reflexivity.
+    unfold shiftR1 in *.
+    simpl.
+ simpl in *.
+    unfold shiftR1. simpl.
+
+  Qed.
+  *)
+
+  Theorem nth_order_shiftout_eq : forall (A : Type)(n : nat)(v : Vec (S n) A) n' (nlt : n' < n)(nlt' :n' < S n),
+    nth_order (shiftout v) nlt = nth_order v nlt'.
+
+    induction n; intros; simpl in *.
+    lia.
+    
+
+    intros.
+    destruct (Vec_S_cons v).
+    destruct H.
+    subst.
+    
+    destruct n'.
+    reflexivity.
+    
+    assert (n' < S n) by lia.
+    erewrite (@nth_order_S_cons _ _ _ _ _ _ H).
+    replace (shiftout (cons A x _ x0)) with (cons A x _ (shiftout x0)).
+    erewrite (@nth_order_S_cons _ _ _ _ _ _).
+    eapply IHn.
+    reflexivity.
+
+    Unshelve.
+    lia.
+    
+  Qed.
+
+  Theorem nth_order_shiftR1_eq : forall (A : Type)(n : nat)(v : Vec n A) n' (nlt : n' < n)(nlt' : pred n' < n) a,
+    n' <> 0%nat ->
+    nth_order (shiftR1 _ _ a v) nlt = nth_order v nlt'.
+
+  (*
+    intros.
+    unfold shiftR1.
+    destruct n.
+    lia.
+    simpl.
+    destruct n'. 
+    lia.
+    
+    Search nth_order cons.
+    assert (n' < n) by lia.
+    rewrite (@nth_order_S_cons A a0 n (shiftout v) n' nlt H0).
+
+    induction v; intros.
+    lia.
+    unfold shiftR1.
+    unfold shiftout.
+    simpl.
+    *)
   Admitted.
 
   Theorem mul_body_equiv : forall pred_wsize p a1 a2 b1 b2,
@@ -2146,6 +2682,17 @@ Section ECEqProof.
     removeCoerce.
     simpl.
     
+    assert (63 < 64)%nat by lia.
+    eapply (sbvToInt_nz_nth _ H0).
+    Search nth_order append.
+    assert (15 < 16) by lia.
+    erewrite (@nth_order_append_eq Bool _ 16 _ 48 (intToBv 48 0) 15 H0 H2).
+    rewrite nth_order_bvAnd_eq.
+    Search shiftR.
+    unfold shiftR.
+    unfold shiftR1.
+    Search nth_order bvAnd.
+    Search sbvToInt.
     (* probably need to add assumption that the integer is a window, so it is in the right range *)
     admit.
 
@@ -2215,24 +2762,11 @@ Section ECEqProof.
 
   Admitted.
 
-  Theorem last_nth_equiv_gen
-     : forall (A : Type) (def : A) (ls : list A) n,
-      n = (Nat.pred (Datatypes.length ls)) ->
-       List.last ls def =
-       List.nth n ls
-         def.
-
-    intros. 
-    subst.
-    apply last_nth_equiv.
-
-  Qed.
-
-
   Definition fiat_point_mul_gen := fiat_point_mul_gen Fsquare Fmul Fsub Fadd Fopp.
 
   Theorem fiat_point_mul_gen_signedRegular_cases : forall wsize numWindows n p,
     0 < wsize < 16 ->
+    (* sbvToInt _ n = bvToInt _ n -> *)
     (BinInt.Z.of_nat (bvToNat 384%nat n) <
  BinInt.Z.shiftl 1 (BinInt.Z.of_nat (S (S (S numWindows)) * wsize)))%Z->
     jac_eq
@@ -2292,19 +2826,7 @@ Section ECEqProof.
     ).
     replace (bvNat 16 0%nat) with (intToBv 16 0%Z).
     rewrite map_nth.
-(*
-    replace (sign_extend_16_64
-           (bvSShr 15
-              (intToBv 16
-                 (List.nth (S (S numWindows))
-                    (recode_rwnaf wsize (S (S (S numWindows)))
-                       (BinInt.Z.of_nat (bvToNat 384 n))) 0%Z))
-              1))
-    with
-    (bvNat 64 (Z.to_nat (Z.shiftr (List.nth (S (S numWindows))
-                    (recode_rwnaf wsize (S (S (S numWindows)))
-                       (BinInt.Z.of_nat (bvToNat 384 n))) 0%Z) 1))).
-*)
+
     rewrite fiat_select_point_ct_gen_nth_equiv.
     unfold groupMul_signedWindows_fold_body.
     unfold groupAdd_signedWindow.
@@ -2413,6 +2935,7 @@ Section ECEqProof.
     apply fiat_mul_scalar_rwnaf_gen_equiv.
     lia.
     admit.
+    trivial.
     intros.
     assert (b0 = c).
     eapply H2.
@@ -2430,9 +2953,11 @@ Section ECEqProof.
     apply fiat_mul_scalar_rwnaf_gen_equiv.
     lia.
     admit.
+    trivial.
 
     intros.  
     destruct wsize.
+    trivial.
     lia.
     apply mul_body_equiv; trivial.
 
@@ -2446,6 +2971,7 @@ Section ECEqProof.
 
   Theorem fiat_point_mul_gen_signedRegular_equiv : forall wsize numWindows n p,
     0 < wsize < 16 ->
+    (* sbvToInt _ n = bvToInt _ n -> *)
     (BinInt.Z.of_nat (bvToNat 384%nat n) <
  BinInt.Z.shiftl 1 (BinInt.Z.of_nat (S (S (S numWindows)) * wsize)))%Z->
     jac_eq
@@ -2473,7 +2999,7 @@ Section ECEqProof.
     eapply point_add_jac_eq.
     eapply jac_eq_symm.
     eapply fiat_point_mul_gen_signedRegular_cases.
-    specialize (@fiat_point_mul_gen_signedRegular_cases wsize numWindows n p); intros; trivial.
+    trivial.
     trivial.
 
     rewrite fiat_pre_comp_table_gen_nth_0.
